mvp ish

extr/Examples.hs
@@ -1,0 +1,2420 @@
+module Examples where
+
+import qualified Prelude
+
+snd :: ((,) a1 a2) -> a2
+snd p =
+  case p of {
+   (,) _ y -> y}
+
+length :: (([]) a1) -> Prelude.Integer
+length l =
+  case l of {
+   ([]) -> 0;
+   (:) _ l' -> Prelude.succ (length l')}
+
+app :: (([]) a1) -> (([]) a1) -> ([]) a1
+app l m =
+  case l of {
+   ([]) -> m;
+   (:) a l1 -> (:) a (app l1 m)}
+
+sub :: Prelude.Integer -> Prelude.Integer -> Prelude.Integer
+sub = (\n m -> Prelude.max 0 (n Prelude.- m))
+
+eqb :: Prelude.Integer -> Prelude.Integer -> Prelude.Bool
+eqb n m =
+  (\fO fS n -> if n Prelude.== 0 then fO () else fS (n Prelude.- 1))
+    (\_ ->
+    (\fO fS n -> if n Prelude.== 0 then fO () else fS (n Prelude.- 1))
+      (\_ -> Prelude.True)
+      (\_ -> Prelude.False)
+      m)
+    (\n' ->
+    (\fO fS n -> if n Prelude.== 0 then fO () else fS (n Prelude.- 1))
+      (\_ -> Prelude.False)
+      (\m' -> eqb n' m')
+      m)
+    n
+
+leb :: Prelude.Integer -> Prelude.Integer -> Prelude.Bool
+leb n m =
+  (\fO fS n -> if n Prelude.== 0 then fO () else fS (n Prelude.- 1))
+    (\_ -> Prelude.True)
+    (\n' ->
+    (\fO fS n -> if n Prelude.== 0 then fO () else fS (n Prelude.- 1))
+      (\_ -> Prelude.False)
+      (\m' -> leb n' m')
+      m)
+    n
+
+pow :: Prelude.Integer -> Prelude.Integer -> Prelude.Integer
+pow n m =
+  (\fO fS n -> if n Prelude.== 0 then fO () else fS (n Prelude.- 1))
+    (\_ -> Prelude.succ 0)
+    (\m0 -> (Prelude.*) n (pow n m0))
+    m
+
+eqb0 :: Prelude.Bool -> Prelude.Bool -> Prelude.Bool
+eqb0 b1 b2 =
+  case b1 of {
+   Prelude.True -> b2;
+   Prelude.False ->
+    case b2 of {
+     Prelude.True -> Prelude.False;
+     Prelude.False -> Prelude.True}}
+
+data Positive =
+   XI Positive
+ | XO Positive
+ | XH
+
+data N =
+   N0
+ | Npos Positive
+
+succ :: Positive -> Positive
+succ x =
+  case x of {
+   XI p -> XO (succ p);
+   XO p -> XI p;
+   XH -> XO XH}
+
+add :: Positive -> Positive -> Positive
+add x y =
+  case x of {
+   XI p ->
+    case y of {
+     XI q -> XO (add_carry p q);
+     XO q -> XI (add p q);
+     XH -> XO (succ p)};
+   XO p ->
+    case y of {
+     XI q -> XI (add p q);
+     XO q -> XO (add p q);
+     XH -> XI p};
+   XH -> case y of {
+          XI q -> XO (succ q);
+          XO q -> XI q;
+          XH -> XO XH}}
+
+add_carry :: Positive -> Positive -> Positive
+add_carry x y =
+  case x of {
+   XI p ->
+    case y of {
+     XI q -> XI (add_carry p q);
+     XO q -> XO (add_carry p q);
+     XH -> XI (succ p)};
+   XO p ->
+    case y of {
+     XI q -> XO (add_carry p q);
+     XO q -> XI (add p q);
+     XH -> XO (succ p)};
+   XH -> case y of {
+          XI q -> XI (succ q);
+          XO q -> XO (succ q);
+          XH -> XI XH}}
+
+mul :: Positive -> Positive -> Positive
+mul x y =
+  case x of {
+   XI p -> add y (XO (mul p y));
+   XO p -> XO (mul p y);
+   XH -> y}
+
+iter_op :: (a1 -> a1 -> a1) -> Positive -> a1 -> a1
+iter_op op p a =
+  case p of {
+   XI p0 -> op a (iter_op op p0 (op a a));
+   XO p0 -> iter_op op p0 (op a a);
+   XH -> a}
+
+to_nat :: Positive -> Prelude.Integer
+to_nat x =
+  iter_op (Prelude.+) x (Prelude.succ 0)
+
+add0 :: N -> N -> N
+add0 n m =
+  case n of {
+   N0 -> m;
+   Npos p -> case m of {
+              N0 -> n;
+              Npos q -> Npos (add p q)}}
+
+mul0 :: N -> N -> N
+mul0 n m =
+  case n of {
+   N0 -> N0;
+   Npos p -> case m of {
+              N0 -> N0;
+              Npos q -> Npos (mul p q)}}
+
+to_nat0 :: N -> Prelude.Integer
+to_nat0 a =
+  case a of {
+   N0 -> 0;
+   Npos p -> to_nat p}
+
+rev :: (([]) a1) -> ([]) a1
+rev l =
+  case l of {
+   ([]) -> ([]);
+   (:) x l' -> app (rev l') ((:) x ([]))}
+
+map :: (a1 -> a2) -> (([]) a1) -> ([]) a2
+map f l =
+  case l of {
+   ([]) -> ([]);
+   (:) a t -> (:) (f a) (map f t)}
+
+fold_right :: (a2 -> a1 -> a1) -> a1 -> (([]) a2) -> a1
+fold_right f a0 l =
+  case l of {
+   ([]) -> a0;
+   (:) b t -> f b (fold_right f a0 t)}
+
+forallb :: (a1 -> Prelude.Bool) -> (([]) a1) -> Prelude.Bool
+forallb f l =
+  case l of {
+   ([]) -> Prelude.True;
+   (:) a l0 -> (Prelude.&&) (f a) (forallb f l0)}
+
+n_of_digits :: (([]) Prelude.Bool) -> N
+n_of_digits l =
+  case l of {
+   ([]) -> N0;
+   (:) b l' ->
+    add0 (case b of {
+           Prelude.True -> Npos XH;
+           Prelude.False -> N0}) (mul0 (Npos (XO XH)) (n_of_digits l'))}
+
+n_of_ascii :: Prelude.Char -> N
+n_of_ascii a =
+  (\f a -> f (Data.Bits.testBit (Data.Char.ord a) 0)
+              (Data.Bits.testBit (Data.Char.ord a) 1)
+              (Data.Bits.testBit (Data.Char.ord a) 2)
+              (Data.Bits.testBit (Data.Char.ord a) 3)
+              (Data.Bits.testBit (Data.Char.ord a) 4)
+              (Data.Bits.testBit (Data.Char.ord a) 5)
+              (Data.Bits.testBit (Data.Char.ord a) 6)
+              (Data.Bits.testBit (Data.Char.ord a) 7))
+    (\a0 a1 a2 a3 a4 a5 a6 a7 ->
+    n_of_digits ((:) a0 ((:) a1 ((:) a2 ((:) a3 ((:) a4 ((:) a5 ((:) a6 ((:)
+      a7 ([]))))))))))
+    a
+
+nat_of_ascii :: Prelude.Char -> Prelude.Integer
+nat_of_ascii a =
+  to_nat0 (n_of_ascii a)
+
+append :: Prelude.String -> Prelude.String -> Prelude.String
+append s1 s2 =
+  case s1 of {
+   ([]) -> s2;
+   (:) c s1' -> (:) c (append s1' s2)}
+
+data Expr =
+   Let Prelude.String Expr Expr
+ | Var Prelude.String
+ | Lambda Prelude.String Expr
+ | Apply Expr Expr
+ | Cond Expr Expr Expr
+ | Nat Prelude.Integer
+ | Add Expr Expr
+ | Sub Expr Expr
+ | Mul Expr Expr
+ | Bool Prelude.Bool
+ | And Expr Expr
+ | Eq Expr Expr
+
+concat_string_list :: (([]) Prelude.String) -> Prelude.String
+concat_string_list l =
+  case l of {
+   ([]) -> "";
+   (:) h t -> append h (concat_string_list t)}
+
+data Env =
+   EmptyEnv
+ | ExtendEnv Prelude.String Value Env
+data Value =
+   V_Nat Prelude.Integer
+ | V_Bool Prelude.Bool
+ | V_Closure Prelude.String Expr Env
+
+lookup_env :: Prelude.String -> Env -> Prelude.Either Prelude.String Value
+lookup_env varName env =
+  case env of {
+   EmptyEnv -> Prelude.Left
+    (append "(lookup_env) Error: Unbound variable '" (append varName "'"));
+   ExtendEnv name value restEnv ->
+    case ((Prelude.==) :: Prelude.String -> Prelude.String -> Prelude.Bool)
+           varName name of {
+     Prelude.True -> Prelude.Right value;
+     Prelude.False -> lookup_env varName restEnv}}
+
+value_to_string :: Value -> Prelude.String
+value_to_string val =
+  case val of {
+   V_Nat _ -> "V_Nat";
+   V_Bool b ->
+    case b of {
+     Prelude.True -> "V_Bool true";
+     Prelude.False -> "V_Bool false"};
+   V_Closure paramName _ _ -> append "(\206\187" (append paramName ")")}
+
+eval :: Expr -> Env -> Prelude.Integer -> Prelude.Either
+        ((,) ((,) Expr Env) (([]) Prelude.String)) Value
+eval expr env max =
+  (\fO fS n -> if n Prelude.== 0 then fO () else fS (n Prelude.- 1))
+    (\_ -> Prelude.Left ((,) ((,) expr env) ((:)
+    "(eval) Error: Maximum recursion depth exceeded" ([]))))
+    (\max' ->
+    case expr of {
+     Let varName bindExpr bodyExpr ->
+      case eval bindExpr env max' of {
+       Prelude.Left err -> Prelude.Left err;
+       Prelude.Right val -> eval bodyExpr (ExtendEnv varName val env) max'};
+     Var varName ->
+      case lookup_env varName env of {
+       Prelude.Left err -> Prelude.Left ((,) ((,) expr env) ((:)
+        (append "(eval) Error: Unbound variable '" (append varName "'")) ((:)
+        err ([]))));
+       Prelude.Right value -> Prelude.Right value};
+     Lambda paramName bodyExpr -> Prelude.Right (V_Closure paramName (Lambda
+      paramName bodyExpr) env);
+     Apply expr1 expr2 ->
+      case eval expr1 env max' of {
+       Prelude.Left err -> Prelude.Left err;
+       Prelude.Right argValue ->
+        case argValue of {
+         V_Closure _ e _ ->
+          case e of {
+           Let _ _ _ ->
+            case eval expr2 env max' of {
+             Prelude.Left err -> Prelude.Left err;
+             Prelude.Right v ->
+              case v of {
+               V_Closure _ e2 _ ->
+                case e2 of {
+                 Lambda paramName bodyExpr ->
+                  eval bodyExpr (ExtendEnv paramName argValue env) max';
+                 _ -> Prelude.Left ((,) ((,) expr env) ((:)
+                  "Error: Application did not evaluate to a closure" ([])))};
+               _ -> Prelude.Left ((,) ((,) expr env) ((:)
+                "Error: Application did not evaluate to a closure" ([])))}};
+           Var _ ->
+            case eval expr2 env max' of {
+             Prelude.Left err -> Prelude.Left err;
+             Prelude.Right v ->
+              case v of {
+               V_Closure _ e0 _ ->
+                case e0 of {
+                 Lambda paramName bodyExpr ->
+                  eval bodyExpr (ExtendEnv paramName argValue env) max';
+                 _ -> Prelude.Left ((,) ((,) expr env) ((:)
+                  "Error: Application did not evaluate to a closure" ([])))};
+               _ -> Prelude.Left ((,) ((,) expr env) ((:)
+                "Error: Application did not evaluate to a closure" ([])))}};
+           Lambda paramName bodyExpr ->
+            case eval expr2 env max' of {
+             Prelude.Left err -> Prelude.Left err;
+             Prelude.Right argValue0 ->
+              eval bodyExpr (ExtendEnv paramName argValue0 env) max'};
+           Cond _ _ _ ->
+            case eval expr2 env max' of {
+             Prelude.Left err -> Prelude.Left err;
+             Prelude.Right v ->
+              case v of {
+               V_Closure _ e3 _ ->
+                case e3 of {
+                 Lambda paramName bodyExpr ->
+                  eval bodyExpr (ExtendEnv paramName argValue env) max';
+                 _ -> Prelude.Left ((,) ((,) expr env) ((:)
+                  "Error: Application did not evaluate to a closure" ([])))};
+               _ -> Prelude.Left ((,) ((,) expr env) ((:)
+                "Error: Application did not evaluate to a closure" ([])))}};
+           Nat _ ->
+            case eval expr2 env max' of {
+             Prelude.Left err -> Prelude.Left err;
+             Prelude.Right v ->
+              case v of {
+               V_Closure _ e0 _ ->
+                case e0 of {
+                 Lambda paramName bodyExpr ->
+                  eval bodyExpr (ExtendEnv paramName argValue env) max';
+                 _ -> Prelude.Left ((,) ((,) expr env) ((:)
+                  "Error: Application did not evaluate to a closure" ([])))};
+               _ -> Prelude.Left ((,) ((,) expr env) ((:)
+                "Error: Application did not evaluate to a closure" ([])))}};
+           Bool _ ->
+            case eval expr2 env max' of {
+             Prelude.Left err -> Prelude.Left err;
+             Prelude.Right v ->
+              case v of {
+               V_Closure _ e0 _ ->
+                case e0 of {
+                 Lambda paramName bodyExpr ->
+                  eval bodyExpr (ExtendEnv paramName argValue env) max';
+                 _ -> Prelude.Left ((,) ((,) expr env) ((:)
+                  "Error: Application did not evaluate to a closure" ([])))};
+               _ -> Prelude.Left ((,) ((,) expr env) ((:)
+                "Error: Application did not evaluate to a closure" ([])))}};
+           _ ->
+            case eval expr2 env max' of {
+             Prelude.Left err -> Prelude.Left err;
+             Prelude.Right v ->
+              case v of {
+               V_Closure _ e2 _ ->
+                case e2 of {
+                 Lambda paramName bodyExpr ->
+                  eval bodyExpr (ExtendEnv paramName argValue env) max';
+                 _ -> Prelude.Left ((,) ((,) expr env) ((:)
+                  "Error: Application did not evaluate to a closure" ([])))};
+               _ -> Prelude.Left ((,) ((,) expr env) ((:)
+                "Error: Application did not evaluate to a closure" ([])))}}};
+         _ ->
+          case eval expr2 env max' of {
+           Prelude.Left err -> Prelude.Left err;
+           Prelude.Right v ->
+            case v of {
+             V_Closure _ e _ ->
+              case e of {
+               Lambda paramName bodyExpr ->
+                eval bodyExpr (ExtendEnv paramName argValue env) max';
+               _ -> Prelude.Left ((,) ((,) expr env) ((:)
+                "Error: Application did not evaluate to a closure" ([])))};
+             _ -> Prelude.Left ((,) ((,) expr env) ((:)
+              "Error: Application did not evaluate to a closure" ([])))}}}};
+     Cond condExpr trueExpr falseExpr ->
+      case eval condExpr env max' of {
+       Prelude.Left p ->
+        case p of {
+         (,) _ err -> Prelude.Left ((,) ((,) expr env) ((:)
+          "(eval) Error: Condition did not evaluate to a boolean" err))};
+       Prelude.Right val ->
+        case val of {
+         V_Bool b ->
+          case b of {
+           Prelude.True -> eval trueExpr env max';
+           Prelude.False -> eval falseExpr env max'};
+         _ -> Prelude.Left ((,) ((,) expr env) ((:)
+          "(eval) Error: Condition did not evaluate to a boolean" ([])))}};
+     Nat n -> Prelude.Right (V_Nat n);
+     Add e1 e2 ->
+      case eval e1 env max' of {
+       Prelude.Left _ -> Prelude.Left ((,) ((,) expr env) ((:)
+        "Error: Addition did not evaluate to a number" ([])));
+       Prelude.Right v ->
+        case v of {
+         V_Nat n1 ->
+          case eval e2 env max' of {
+           Prelude.Left _ -> Prelude.Left ((,) ((,) expr env) ((:)
+            "Error: Addition did not evaluate to a number" ([])));
+           Prelude.Right v0 ->
+            case v0 of {
+             V_Nat n2 -> Prelude.Right (V_Nat ((Prelude.+) n1 n2));
+             _ -> Prelude.Left ((,) ((,) expr env) ((:)
+              "Error: Addition did not evaluate to a number" ([])))}};
+         _ -> Prelude.Left ((,) ((,) expr env) ((:)
+          "Error: Addition did not evaluate to a number" ([])))}};
+     Sub e1 e2 ->
+      case eval e1 env max' of {
+       Prelude.Left _ -> Prelude.Left ((,) ((,) expr env) ((:)
+        "Error: Subtraction did not evaluate to a number" ([])));
+       Prelude.Right v ->
+        case v of {
+         V_Nat n1 ->
+          case eval e2 env max' of {
+           Prelude.Left _ -> Prelude.Left ((,) ((,) expr env) ((:)
+            "Error: Subtraction did not evaluate to a number" ([])));
+           Prelude.Right v0 ->
+            case v0 of {
+             V_Nat n2 -> Prelude.Right (V_Nat (sub n1 n2));
+             _ -> Prelude.Left ((,) ((,) expr env) ((:)
+              "Error: Subtraction did not evaluate to a number" ([])))}};
+         _ -> Prelude.Left ((,) ((,) expr env) ((:)
+          "Error: Subtraction did not evaluate to a number" ([])))}};
+     Mul e1 e2 ->
+      case eval e1 env max' of {
+       Prelude.Left p ->
+        case p of {
+         (,) _ err ->
+          case eval e2 env max' of {
+           Prelude.Left _ -> Prelude.Left ((,) ((,) expr env) ((:)
+            "E4rror: Multiplication did not evaluate to a number" ([])));
+           Prelude.Right val -> Prelude.Left ((,) ((,) expr env) ((:)
+            (append "3Error: Multiplication did not evaluate to a number: "
+              (value_to_string val)) err))}};
+       Prelude.Right val ->
+        case val of {
+         V_Nat n1 ->
+          case eval e2 env max' of {
+           Prelude.Left p ->
+            case p of {
+             (,) _ err -> Prelude.Left ((,) ((,) expr env) ((:)
+              (append "2Error: Multiplication did not evaluate to a number: "
+                (value_to_string val)) err))};
+           Prelude.Right val' ->
+            case val' of {
+             V_Nat n2 -> Prelude.Right (V_Nat ((Prelude.*) n1 n2));
+             V_Bool _ -> Prelude.Left ((,) ((,) expr env) ((:)
+              (append "1Error: Multiplication did not evaluate to a number: "
+                (append (value_to_string val) (value_to_string val'))) ([])));
+             V_Closure paramName bodyExpr closureEnv -> Prelude.Right
+              (V_Closure paramName (Mul (Nat n1) bodyExpr) closureEnv)}};
+         V_Bool _ ->
+          case eval e2 env max' of {
+           Prelude.Left p ->
+            case p of {
+             (,) _ err -> Prelude.Left ((,) ((,) expr env) ((:)
+              (append "2Error: Multiplication did not evaluate to a number: "
+                (value_to_string val)) err))};
+           Prelude.Right val' -> Prelude.Left ((,) ((,) expr env) ((:)
+            (append "1Error: Multiplication did not evaluate to a number: "
+              (append (value_to_string val) (value_to_string val'))) ([])))};
+         V_Closure paramName1 bodyExpr1 closureEnv1 ->
+          case eval e2 env max' of {
+           Prelude.Left p ->
+            case p of {
+             (,) _ err -> Prelude.Left ((,) ((,) expr env) ((:)
+              (append "2Error: Multiplication did not evaluate to a number: "
+                (value_to_string val)) err))};
+           Prelude.Right val' ->
+            case val' of {
+             V_Nat n2 -> Prelude.Right (V_Closure paramName1 (Mul bodyExpr1
+              (Nat n2)) closureEnv1);
+             V_Bool _ -> Prelude.Left ((,) ((,) expr env) ((:)
+              (append "1Error: Multiplication did not evaluate to a number: "
+                (append (value_to_string val) (value_to_string val'))) ([])));
+             V_Closure _ bodyExpr2 _ -> Prelude.Right (V_Closure paramName1
+              (Mul bodyExpr1 (Apply bodyExpr2 (Var paramName1))) closureEnv1)}}}};
+     Bool b -> Prelude.Right (V_Bool b);
+     And e1 e2 ->
+      case eval e1 env max' of {
+       Prelude.Left _ -> Prelude.Left ((,) ((,) expr env) ((:)
+        "Error: And did not evaluate to a boolean" ([])));
+       Prelude.Right v ->
+        case v of {
+         V_Bool b1 ->
+          case eval e2 env max' of {
+           Prelude.Left _ -> Prelude.Left ((,) ((,) expr env) ((:)
+            "Error: And did not evaluate to a boolean" ([])));
+           Prelude.Right v0 ->
+            case v0 of {
+             V_Bool b2 -> Prelude.Right (V_Bool ((Prelude.&&) b1 b2));
+             _ -> Prelude.Left ((,) ((,) expr env) ((:)
+              "Error: And did not evaluate to a boolean" ([])))}};
+         _ -> Prelude.Left ((,) ((,) expr env) ((:)
+          "Error: And did not evaluate to a boolean" ([])))}};
+     Eq e1 e2 ->
+      case eval e1 env max' of {
+       Prelude.Left _ -> Prelude.Left ((,) ((,) expr env) ((:)
+        "Error: Cannot compare values of non-equal types" ([])));
+       Prelude.Right v ->
+        case v of {
+         V_Nat n1 ->
+          case eval e2 env max' of {
+           Prelude.Left _ -> Prelude.Left ((,) ((,) expr env) ((:)
+            "Error: Cannot compare values of non-equal types" ([])));
+           Prelude.Right v0 ->
+            case v0 of {
+             V_Nat n2 -> Prelude.Right (V_Bool (eqb n1 n2));
+             _ -> Prelude.Left ((,) ((,) expr env) ((:)
+              "Error: Cannot compare values of non-equal types" ([])))}};
+         V_Bool b1 ->
+          case eval e2 env max' of {
+           Prelude.Left _ -> Prelude.Left ((,) ((,) expr env) ((:)
+            "Error: Cannot compare values of non-equal types" ([])));
+           Prelude.Right v0 ->
+            case v0 of {
+             V_Bool b2 -> Prelude.Right (V_Bool (eqb0 b1 b2));
+             _ -> Prelude.Left ((,) ((,) expr env) ((:)
+              "Error: Cannot compare values of non-equal types" ([])))}};
+         V_Closure _ _ _ -> Prelude.Left ((,) ((,) expr env) ((:)
+          "Error: Cannot compare values of non-equal types" ([])))}}})
+    max
+
+isWhite :: Prelude.Char -> Prelude.Bool
+isWhite c =
+  let {n = nat_of_ascii c} in
+  (Prelude.||)
+    ((Prelude.||)
+      (eqb n (Prelude.succ (Prelude.succ (Prelude.succ (Prelude.succ
+        (Prelude.succ (Prelude.succ (Prelude.succ (Prelude.succ (Prelude.succ
+        (Prelude.succ (Prelude.succ (Prelude.succ (Prelude.succ (Prelude.succ
+        (Prelude.succ (Prelude.succ (Prelude.succ (Prelude.succ (Prelude.succ
+        (Prelude.succ (Prelude.succ (Prelude.succ (Prelude.succ (Prelude.succ
+        (Prelude.succ (Prelude.succ (Prelude.succ (Prelude.succ (Prelude.succ
+        (Prelude.succ (Prelude.succ (Prelude.succ
+        0)))))))))))))))))))))))))))))))))
+      (eqb n (Prelude.succ (Prelude.succ (Prelude.succ (Prelude.succ
+        (Prelude.succ (Prelude.succ (Prelude.succ (Prelude.succ (Prelude.succ
+        0)))))))))))
+    ((Prelude.||)
+      (eqb n (Prelude.succ (Prelude.succ (Prelude.succ (Prelude.succ
+        (Prelude.succ (Prelude.succ (Prelude.succ (Prelude.succ (Prelude.succ
+        (Prelude.succ 0)))))))))))
+      (eqb n (Prelude.succ (Prelude.succ (Prelude.succ (Prelude.succ
+        (Prelude.succ (Prelude.succ (Prelude.succ (Prelude.succ (Prelude.succ
+        (Prelude.succ (Prelude.succ (Prelude.succ (Prelude.succ
+        0)))))))))))))))
+
+isLowerAlpha :: Prelude.Char -> Prelude.Bool
+isLowerAlpha c =
+  let {n = nat_of_ascii c} in
+  (Prelude.&&)
+    (leb (Prelude.succ (Prelude.succ (Prelude.succ (Prelude.succ
+      (Prelude.succ (Prelude.succ (Prelude.succ (Prelude.succ (Prelude.succ
+      (Prelude.succ (Prelude.succ (Prelude.succ (Prelude.succ (Prelude.succ
+      (Prelude.succ (Prelude.succ (Prelude.succ (Prelude.succ (Prelude.succ
+      (Prelude.succ (Prelude.succ (Prelude.succ (Prelude.succ (Prelude.succ
+      (Prelude.succ (Prelude.succ (Prelude.succ (Prelude.succ (Prelude.succ
+      (Prelude.succ (Prelude.succ (Prelude.succ (Prelude.succ (Prelude.succ
+      (Prelude.succ (Prelude.succ (Prelude.succ (Prelude.succ (Prelude.succ
+      (Prelude.succ (Prelude.succ (Prelude.succ (Prelude.succ (Prelude.succ
+      (Prelude.succ (Prelude.succ (Prelude.succ (Prelude.succ (Prelude.succ
+      (Prelude.succ (Prelude.succ (Prelude.succ (Prelude.succ (Prelude.succ
+      (Prelude.succ (Prelude.succ (Prelude.succ (Prelude.succ (Prelude.succ
+      (Prelude.succ (Prelude.succ (Prelude.succ (Prelude.succ (Prelude.succ
+      (Prelude.succ (Prelude.succ (Prelude.succ (Prelude.succ (Prelude.succ
+      (Prelude.succ (Prelude.succ (Prelude.succ (Prelude.succ (Prelude.succ
+      (Prelude.succ (Prelude.succ (Prelude.succ (Prelude.succ (Prelude.succ
+      (Prelude.succ (Prelude.succ (Prelude.succ (Prelude.succ (Prelude.succ
+      (Prelude.succ (Prelude.succ (Prelude.succ (Prelude.succ (Prelude.succ
+      (Prelude.succ (Prelude.succ (Prelude.succ (Prelude.succ (Prelude.succ
+      (Prelude.succ (Prelude.succ (Prelude.succ
+      0)))))))))))))))))))))))))))))))))))))))))))))))))))))))))))))))))))))))))))))))))))))))))))))))))
+      n)
+    (leb n (Prelude.succ (Prelude.succ (Prelude.succ (Prelude.succ
+      (Prelude.succ (Prelude.succ (Prelude.succ (Prelude.succ (Prelude.succ
+      (Prelude.succ (Prelude.succ (Prelude.succ (Prelude.succ (Prelude.succ
+      (Prelude.succ (Prelude.succ (Prelude.succ (Prelude.succ (Prelude.succ
+      (Prelude.succ (Prelude.succ (Prelude.succ (Prelude.succ (Prelude.succ
+      (Prelude.succ (Prelude.succ (Prelude.succ (Prelude.succ (Prelude.succ
+      (Prelude.succ (Prelude.succ (Prelude.succ (Prelude.succ (Prelude.succ
+      (Prelude.succ (Prelude.succ (Prelude.succ (Prelude.succ (Prelude.succ
+      (Prelude.succ (Prelude.succ (Prelude.succ (Prelude.succ (Prelude.succ
+      (Prelude.succ (Prelude.succ (Prelude.succ (Prelude.succ (Prelude.succ
+      (Prelude.succ (Prelude.succ (Prelude.succ (Prelude.succ (Prelude.succ
+      (Prelude.succ (Prelude.succ (Prelude.succ (Prelude.succ (Prelude.succ
+      (Prelude.succ (Prelude.succ (Prelude.succ (Prelude.succ (Prelude.succ
+      (Prelude.succ (Prelude.succ (Prelude.succ (Prelude.succ (Prelude.succ
+      (Prelude.succ (Prelude.succ (Prelude.succ (Prelude.succ (Prelude.succ
+      (Prelude.succ (Prelude.succ (Prelude.succ (Prelude.succ (Prelude.succ
+      (Prelude.succ (Prelude.succ (Prelude.succ (Prelude.succ (Prelude.succ
+      (Prelude.succ (Prelude.succ (Prelude.succ (Prelude.succ (Prelude.succ
+      (Prelude.succ (Prelude.succ (Prelude.succ (Prelude.succ (Prelude.succ
+      (Prelude.succ (Prelude.succ (Prelude.succ (Prelude.succ (Prelude.succ
+      (Prelude.succ (Prelude.succ (Prelude.succ (Prelude.succ (Prelude.succ
+      (Prelude.succ (Prelude.succ (Prelude.succ (Prelude.succ (Prelude.succ
+      (Prelude.succ (Prelude.succ (Prelude.succ (Prelude.succ (Prelude.succ
+      (Prelude.succ (Prelude.succ (Prelude.succ (Prelude.succ (Prelude.succ
+      (Prelude.succ (Prelude.succ (Prelude.succ
+      0)))))))))))))))))))))))))))))))))))))))))))))))))))))))))))))))))))))))))))))))))))))))))))))))))))))))))))))))))))))))))))
+
+isAlpha :: Prelude.Char -> Prelude.Bool
+isAlpha c =
+  let {n = nat_of_ascii c} in
+  (Prelude.||)
+    ((Prelude.&&)
+      (leb (Prelude.succ (Prelude.succ (Prelude.succ (Prelude.succ
+        (Prelude.succ (Prelude.succ (Prelude.succ (Prelude.succ (Prelude.succ
+        (Prelude.succ (Prelude.succ (Prelude.succ (Prelude.succ (Prelude.succ
+        (Prelude.succ (Prelude.succ (Prelude.succ (Prelude.succ (Prelude.succ
+        (Prelude.succ (Prelude.succ (Prelude.succ (Prelude.succ (Prelude.succ
+        (Prelude.succ (Prelude.succ (Prelude.succ (Prelude.succ (Prelude.succ
+        (Prelude.succ (Prelude.succ (Prelude.succ (Prelude.succ (Prelude.succ
+        (Prelude.succ (Prelude.succ (Prelude.succ (Prelude.succ (Prelude.succ
+        (Prelude.succ (Prelude.succ (Prelude.succ (Prelude.succ (Prelude.succ
+        (Prelude.succ (Prelude.succ (Prelude.succ (Prelude.succ (Prelude.succ
+        (Prelude.succ (Prelude.succ (Prelude.succ (Prelude.succ (Prelude.succ
+        (Prelude.succ (Prelude.succ (Prelude.succ (Prelude.succ (Prelude.succ
+        (Prelude.succ (Prelude.succ (Prelude.succ (Prelude.succ (Prelude.succ
+        (Prelude.succ
+        0))))))))))))))))))))))))))))))))))))))))))))))))))))))))))))))))) n)
+      (leb n (Prelude.succ (Prelude.succ (Prelude.succ (Prelude.succ
+        (Prelude.succ (Prelude.succ (Prelude.succ (Prelude.succ (Prelude.succ
+        (Prelude.succ (Prelude.succ (Prelude.succ (Prelude.succ (Prelude.succ
+        (Prelude.succ (Prelude.succ (Prelude.succ (Prelude.succ (Prelude.succ
+        (Prelude.succ (Prelude.succ (Prelude.succ (Prelude.succ (Prelude.succ
+        (Prelude.succ (Prelude.succ (Prelude.succ (Prelude.succ (Prelude.succ
+        (Prelude.succ (Prelude.succ (Prelude.succ (Prelude.succ (Prelude.succ
+        (Prelude.succ (Prelude.succ (Prelude.succ (Prelude.succ (Prelude.succ
+        (Prelude.succ (Prelude.succ (Prelude.succ (Prelude.succ (Prelude.succ
+        (Prelude.succ (Prelude.succ (Prelude.succ (Prelude.succ (Prelude.succ
+        (Prelude.succ (Prelude.succ (Prelude.succ (Prelude.succ (Prelude.succ
+        (Prelude.succ (Prelude.succ (Prelude.succ (Prelude.succ (Prelude.succ
+        (Prelude.succ (Prelude.succ (Prelude.succ (Prelude.succ (Prelude.succ
+        (Prelude.succ (Prelude.succ (Prelude.succ (Prelude.succ (Prelude.succ
+        (Prelude.succ (Prelude.succ (Prelude.succ (Prelude.succ (Prelude.succ
+        (Prelude.succ (Prelude.succ (Prelude.succ (Prelude.succ (Prelude.succ
+        (Prelude.succ (Prelude.succ (Prelude.succ (Prelude.succ (Prelude.succ
+        (Prelude.succ (Prelude.succ (Prelude.succ (Prelude.succ (Prelude.succ
+        (Prelude.succ
+        0))))))))))))))))))))))))))))))))))))))))))))))))))))))))))))))))))))))))))))))))))))))))))))
+    ((Prelude.&&)
+      (leb (Prelude.succ (Prelude.succ (Prelude.succ (Prelude.succ
+        (Prelude.succ (Prelude.succ (Prelude.succ (Prelude.succ (Prelude.succ
+        (Prelude.succ (Prelude.succ (Prelude.succ (Prelude.succ (Prelude.succ
+        (Prelude.succ (Prelude.succ (Prelude.succ (Prelude.succ (Prelude.succ
+        (Prelude.succ (Prelude.succ (Prelude.succ (Prelude.succ (Prelude.succ
+        (Prelude.succ (Prelude.succ (Prelude.succ (Prelude.succ (Prelude.succ
+        (Prelude.succ (Prelude.succ (Prelude.succ (Prelude.succ (Prelude.succ
+        (Prelude.succ (Prelude.succ (Prelude.succ (Prelude.succ (Prelude.succ
+        (Prelude.succ (Prelude.succ (Prelude.succ (Prelude.succ (Prelude.succ
+        (Prelude.succ (Prelude.succ (Prelude.succ (Prelude.succ (Prelude.succ
+        (Prelude.succ (Prelude.succ (Prelude.succ (Prelude.succ (Prelude.succ
+        (Prelude.succ (Prelude.succ (Prelude.succ (Prelude.succ (Prelude.succ
+        (Prelude.succ (Prelude.succ (Prelude.succ (Prelude.succ (Prelude.succ
+        (Prelude.succ (Prelude.succ (Prelude.succ (Prelude.succ (Prelude.succ
+        (Prelude.succ (Prelude.succ (Prelude.succ (Prelude.succ (Prelude.succ
+        (Prelude.succ (Prelude.succ (Prelude.succ (Prelude.succ (Prelude.succ
+        (Prelude.succ (Prelude.succ (Prelude.succ (Prelude.succ (Prelude.succ
+        (Prelude.succ (Prelude.succ (Prelude.succ (Prelude.succ (Prelude.succ
+        (Prelude.succ (Prelude.succ (Prelude.succ (Prelude.succ (Prelude.succ
+        (Prelude.succ (Prelude.succ (Prelude.succ
+        0)))))))))))))))))))))))))))))))))))))))))))))))))))))))))))))))))))))))))))))))))))))))))))))))))
+        n)
+      (leb n (Prelude.succ (Prelude.succ (Prelude.succ (Prelude.succ
+        (Prelude.succ (Prelude.succ (Prelude.succ (Prelude.succ (Prelude.succ
+        (Prelude.succ (Prelude.succ (Prelude.succ (Prelude.succ (Prelude.succ
+        (Prelude.succ (Prelude.succ (Prelude.succ (Prelude.succ (Prelude.succ
+        (Prelude.succ (Prelude.succ (Prelude.succ (Prelude.succ (Prelude.succ
+        (Prelude.succ (Prelude.succ (Prelude.succ (Prelude.succ (Prelude.succ
+        (Prelude.succ (Prelude.succ (Prelude.succ (Prelude.succ (Prelude.succ
+        (Prelude.succ (Prelude.succ (Prelude.succ (Prelude.succ (Prelude.succ
+        (Prelude.succ (Prelude.succ (Prelude.succ (Prelude.succ (Prelude.succ
+        (Prelude.succ (Prelude.succ (Prelude.succ (Prelude.succ (Prelude.succ
+        (Prelude.succ (Prelude.succ (Prelude.succ (Prelude.succ (Prelude.succ
+        (Prelude.succ (Prelude.succ (Prelude.succ (Prelude.succ (Prelude.succ
+        (Prelude.succ (Prelude.succ (Prelude.succ (Prelude.succ (Prelude.succ
+        (Prelude.succ (Prelude.succ (Prelude.succ (Prelude.succ (Prelude.succ
+        (Prelude.succ (Prelude.succ (Prelude.succ (Prelude.succ (Prelude.succ
+        (Prelude.succ (Prelude.succ (Prelude.succ (Prelude.succ (Prelude.succ
+        (Prelude.succ (Prelude.succ (Prelude.succ (Prelude.succ (Prelude.succ
+        (Prelude.succ (Prelude.succ (Prelude.succ (Prelude.succ (Prelude.succ
+        (Prelude.succ (Prelude.succ (Prelude.succ (Prelude.succ (Prelude.succ
+        (Prelude.succ (Prelude.succ (Prelude.succ (Prelude.succ (Prelude.succ
+        (Prelude.succ (Prelude.succ (Prelude.succ (Prelude.succ (Prelude.succ
+        (Prelude.succ (Prelude.succ (Prelude.succ (Prelude.succ (Prelude.succ
+        (Prelude.succ (Prelude.succ (Prelude.succ (Prelude.succ (Prelude.succ
+        (Prelude.succ (Prelude.succ (Prelude.succ (Prelude.succ (Prelude.succ
+        (Prelude.succ (Prelude.succ (Prelude.succ
+        0))))))))))))))))))))))))))))))))))))))))))))))))))))))))))))))))))))))))))))))))))))))))))))))))))))))))))))))))))))))))))))
+
+isDigit :: Prelude.Char -> Prelude.Bool
+isDigit c =
+  let {n = nat_of_ascii c} in
+  (Prelude.&&)
+    (leb (Prelude.succ (Prelude.succ (Prelude.succ (Prelude.succ
+      (Prelude.succ (Prelude.succ (Prelude.succ (Prelude.succ (Prelude.succ
+      (Prelude.succ (Prelude.succ (Prelude.succ (Prelude.succ (Prelude.succ
+      (Prelude.succ (Prelude.succ (Prelude.succ (Prelude.succ (Prelude.succ
+      (Prelude.succ (Prelude.succ (Prelude.succ (Prelude.succ (Prelude.succ
+      (Prelude.succ (Prelude.succ (Prelude.succ (Prelude.succ (Prelude.succ
+      (Prelude.succ (Prelude.succ (Prelude.succ (Prelude.succ (Prelude.succ
+      (Prelude.succ (Prelude.succ (Prelude.succ (Prelude.succ (Prelude.succ
+      (Prelude.succ (Prelude.succ (Prelude.succ (Prelude.succ (Prelude.succ
+      (Prelude.succ (Prelude.succ (Prelude.succ (Prelude.succ
+      0)))))))))))))))))))))))))))))))))))))))))))))))) n)
+    (leb n (Prelude.succ (Prelude.succ (Prelude.succ (Prelude.succ
+      (Prelude.succ (Prelude.succ (Prelude.succ (Prelude.succ (Prelude.succ
+      (Prelude.succ (Prelude.succ (Prelude.succ (Prelude.succ (Prelude.succ
+      (Prelude.succ (Prelude.succ (Prelude.succ (Prelude.succ (Prelude.succ
+      (Prelude.succ (Prelude.succ (Prelude.succ (Prelude.succ (Prelude.succ
+      (Prelude.succ (Prelude.succ (Prelude.succ (Prelude.succ (Prelude.succ
+      (Prelude.succ (Prelude.succ (Prelude.succ (Prelude.succ (Prelude.succ
+      (Prelude.succ (Prelude.succ (Prelude.succ (Prelude.succ (Prelude.succ
+      (Prelude.succ (Prelude.succ (Prelude.succ (Prelude.succ (Prelude.succ
+      (Prelude.succ (Prelude.succ (Prelude.succ (Prelude.succ (Prelude.succ
+      (Prelude.succ (Prelude.succ (Prelude.succ (Prelude.succ (Prelude.succ
+      (Prelude.succ (Prelude.succ (Prelude.succ
+      0))))))))))))))))))))))))))))))))))))))))))))))))))))))))))
+
+data Chartype =
+   White
+ | Alpha
+ | Digit
+ | Other
+
+classifyChar :: Prelude.Char -> Chartype
+classifyChar c =
+  case isWhite c of {
+   Prelude.True -> White;
+   Prelude.False ->
+    case isAlpha c of {
+     Prelude.True -> Alpha;
+     Prelude.False ->
+      case isDigit c of {
+       Prelude.True -> Digit;
+       Prelude.False -> Other}}}
+
+list_of_string :: Prelude.String -> ([]) Prelude.Char
+list_of_string s =
+  case s of {
+   ([]) -> ([]);
+   (:) c s0 -> (:) c (list_of_string s0)}
+
+string_of_list :: (([]) Prelude.Char) -> Prelude.String
+string_of_list xs =
+  fold_right (\x x0 -> (:) x x0) "" xs
+
+string_to_nat' :: (([]) Prelude.Char) -> Prelude.Integer -> Prelude.Maybe
+                  Prelude.Integer
+string_to_nat' cs len =
+  case cs of {
+   ([]) -> Prelude.Just 0;
+   (:) h t ->
+    case classifyChar h of {
+     Digit ->
+      case string_to_nat' t (sub len (Prelude.succ 0)) of {
+       Prelude.Just n -> Prelude.Just
+        ((Prelude.+)
+          ((Prelude.*)
+            (pow (Prelude.succ (Prelude.succ (Prelude.succ (Prelude.succ
+              (Prelude.succ (Prelude.succ (Prelude.succ (Prelude.succ
+              (Prelude.succ (Prelude.succ 0))))))))))
+              (sub len (Prelude.succ 0)))
+            (sub (nat_of_ascii h) (Prelude.succ (Prelude.succ (Prelude.succ
+              (Prelude.succ (Prelude.succ (Prelude.succ (Prelude.succ
+              (Prelude.succ (Prelude.succ (Prelude.succ (Prelude.succ
+              (Prelude.succ (Prelude.succ (Prelude.succ (Prelude.succ
+              (Prelude.succ (Prelude.succ (Prelude.succ (Prelude.succ
+              (Prelude.succ (Prelude.succ (Prelude.succ (Prelude.succ
+              (Prelude.succ (Prelude.succ (Prelude.succ (Prelude.succ
+              (Prelude.succ (Prelude.succ (Prelude.succ (Prelude.succ
+              (Prelude.succ (Prelude.succ (Prelude.succ (Prelude.succ
+              (Prelude.succ (Prelude.succ (Prelude.succ (Prelude.succ
+              (Prelude.succ (Prelude.succ (Prelude.succ (Prelude.succ
+              (Prelude.succ (Prelude.succ (Prelude.succ (Prelude.succ
+              (Prelude.succ
+              0)))))))))))))))))))))))))))))))))))))))))))))))))) n);
+       Prelude.Nothing -> Prelude.Nothing};
+     _ -> Prelude.Nothing}}
+
+string_to_nat :: Prelude.String -> Prelude.Maybe Prelude.Integer
+string_to_nat s =
+  let {char_list = list_of_string s} in
+  let {len = length char_list} in string_to_nat' char_list len
+
+tokenize_helper :: Chartype -> (([]) Prelude.Char) -> (([]) Prelude.Char) ->
+                   ([]) (([]) Prelude.Char)
+tokenize_helper cls acc xs =
+  let {tk = case acc of {
+             ([]) -> ([]);
+             (:) _ _ -> (:) (rev acc) ([])}} in
+  case xs of {
+   ([]) -> tk;
+   (:) x xs' ->
+    case cls of {
+     White ->
+      case classifyChar x of {
+       White ->
+        (\f a -> f (Data.Bits.testBit (Data.Char.ord a) 0)
+              (Data.Bits.testBit (Data.Char.ord a) 1)
+              (Data.Bits.testBit (Data.Char.ord a) 2)
+              (Data.Bits.testBit (Data.Char.ord a) 3)
+              (Data.Bits.testBit (Data.Char.ord a) 4)
+              (Data.Bits.testBit (Data.Char.ord a) 5)
+              (Data.Bits.testBit (Data.Char.ord a) 6)
+              (Data.Bits.testBit (Data.Char.ord a) 7))
+          (\b b0 b1 b2 b3 b4 b5 b6 ->
+          case b of {
+           Prelude.True ->
+            case b0 of {
+             Prelude.True -> app tk (tokenize_helper White ([]) xs');
+             Prelude.False ->
+              case b1 of {
+               Prelude.True -> app tk (tokenize_helper White ([]) xs');
+               Prelude.False ->
+                case b2 of {
+                 Prelude.True ->
+                  case b3 of {
+                   Prelude.True -> app tk (tokenize_helper White ([]) xs');
+                   Prelude.False ->
+                    case b4 of {
+                     Prelude.True ->
+                      case b5 of {
+                       Prelude.True ->
+                        app tk (tokenize_helper White ([]) xs');
+                       Prelude.False ->
+                        case b6 of {
+                         Prelude.True ->
+                          app tk (tokenize_helper White ([]) xs');
+                         Prelude.False ->
+                          app tk ((:) ((:) ')' ([]))
+                            (tokenize_helper Other ([]) xs'))}};
+                     Prelude.False -> app tk (tokenize_helper White ([]) xs')}};
+                 Prelude.False -> app tk (tokenize_helper White ([]) xs')}}};
+           Prelude.False ->
+            case b0 of {
+             Prelude.True -> app tk (tokenize_helper White ([]) xs');
+             Prelude.False ->
+              case b1 of {
+               Prelude.True -> app tk (tokenize_helper White ([]) xs');
+               Prelude.False ->
+                case b2 of {
+                 Prelude.True ->
+                  case b3 of {
+                   Prelude.True -> app tk (tokenize_helper White ([]) xs');
+                   Prelude.False ->
+                    case b4 of {
+                     Prelude.True ->
+                      case b5 of {
+                       Prelude.True ->
+                        app tk (tokenize_helper White ([]) xs');
+                       Prelude.False ->
+                        case b6 of {
+                         Prelude.True ->
+                          app tk (tokenize_helper White ([]) xs');
+                         Prelude.False ->
+                          app tk ((:) ((:) '(' ([]))
+                            (tokenize_helper Other ([]) xs'))}};
+                     Prelude.False -> app tk (tokenize_helper White ([]) xs')}};
+                 Prelude.False -> app tk (tokenize_helper White ([]) xs')}}}})
+          x;
+       Other ->
+        let {tp = Other} in
+        (\f a -> f (Data.Bits.testBit (Data.Char.ord a) 0)
+              (Data.Bits.testBit (Data.Char.ord a) 1)
+              (Data.Bits.testBit (Data.Char.ord a) 2)
+              (Data.Bits.testBit (Data.Char.ord a) 3)
+              (Data.Bits.testBit (Data.Char.ord a) 4)
+              (Data.Bits.testBit (Data.Char.ord a) 5)
+              (Data.Bits.testBit (Data.Char.ord a) 6)
+              (Data.Bits.testBit (Data.Char.ord a) 7))
+          (\b b0 b1 b2 b3 b4 b5 b6 ->
+          case b of {
+           Prelude.True ->
+            case b0 of {
+             Prelude.True -> app tk (tokenize_helper tp ((:) x ([])) xs');
+             Prelude.False ->
+              case b1 of {
+               Prelude.True -> app tk (tokenize_helper tp ((:) x ([])) xs');
+               Prelude.False ->
+                case b2 of {
+                 Prelude.True ->
+                  case b3 of {
+                   Prelude.True ->
+                    app tk (tokenize_helper tp ((:) x ([])) xs');
+                   Prelude.False ->
+                    case b4 of {
+                     Prelude.True ->
+                      case b5 of {
+                       Prelude.True ->
+                        app tk (tokenize_helper tp ((:) x ([])) xs');
+                       Prelude.False ->
+                        case b6 of {
+                         Prelude.True ->
+                          app tk (tokenize_helper tp ((:) x ([])) xs');
+                         Prelude.False ->
+                          app tk ((:) ((:) ')' ([]))
+                            (tokenize_helper Other ([]) xs'))}};
+                     Prelude.False ->
+                      app tk (tokenize_helper tp ((:) x ([])) xs')}};
+                 Prelude.False ->
+                  app tk (tokenize_helper tp ((:) x ([])) xs')}}};
+           Prelude.False ->
+            case b0 of {
+             Prelude.True -> app tk (tokenize_helper tp ((:) x ([])) xs');
+             Prelude.False ->
+              case b1 of {
+               Prelude.True -> app tk (tokenize_helper tp ((:) x ([])) xs');
+               Prelude.False ->
+                case b2 of {
+                 Prelude.True ->
+                  case b3 of {
+                   Prelude.True ->
+                    app tk (tokenize_helper tp ((:) x ([])) xs');
+                   Prelude.False ->
+                    case b4 of {
+                     Prelude.True ->
+                      case b5 of {
+                       Prelude.True ->
+                        app tk (tokenize_helper tp ((:) x ([])) xs');
+                       Prelude.False ->
+                        case b6 of {
+                         Prelude.True ->
+                          app tk (tokenize_helper tp ((:) x ([])) xs');
+                         Prelude.False ->
+                          app tk ((:) ((:) '(' ([]))
+                            (tokenize_helper Other ([]) xs'))}};
+                     Prelude.False ->
+                      app tk (tokenize_helper tp ((:) x ([])) xs')}};
+                 Prelude.False ->
+                  app tk (tokenize_helper tp ((:) x ([])) xs')}}}})
+          x;
+       x0 ->
+        (\f a -> f (Data.Bits.testBit (Data.Char.ord a) 0)
+              (Data.Bits.testBit (Data.Char.ord a) 1)
+              (Data.Bits.testBit (Data.Char.ord a) 2)
+              (Data.Bits.testBit (Data.Char.ord a) 3)
+              (Data.Bits.testBit (Data.Char.ord a) 4)
+              (Data.Bits.testBit (Data.Char.ord a) 5)
+              (Data.Bits.testBit (Data.Char.ord a) 6)
+              (Data.Bits.testBit (Data.Char.ord a) 7))
+          (\b b0 b1 b2 b3 b4 b5 b6 ->
+          case b of {
+           Prelude.True ->
+            case b0 of {
+             Prelude.True -> app tk (tokenize_helper x0 ((:) x ([])) xs');
+             Prelude.False ->
+              case b1 of {
+               Prelude.True -> app tk (tokenize_helper x0 ((:) x ([])) xs');
+               Prelude.False ->
+                case b2 of {
+                 Prelude.True ->
+                  case b3 of {
+                   Prelude.True ->
+                    app tk (tokenize_helper x0 ((:) x ([])) xs');
+                   Prelude.False ->
+                    case b4 of {
+                     Prelude.True ->
+                      case b5 of {
+                       Prelude.True ->
+                        app tk (tokenize_helper x0 ((:) x ([])) xs');
+                       Prelude.False ->
+                        case b6 of {
+                         Prelude.True ->
+                          app tk (tokenize_helper x0 ((:) x ([])) xs');
+                         Prelude.False ->
+                          app tk ((:) ((:) ')' ([]))
+                            (tokenize_helper Other ([]) xs'))}};
+                     Prelude.False ->
+                      app tk (tokenize_helper x0 ((:) x ([])) xs')}};
+                 Prelude.False ->
+                  app tk (tokenize_helper x0 ((:) x ([])) xs')}}};
+           Prelude.False ->
+            case b0 of {
+             Prelude.True -> app tk (tokenize_helper x0 ((:) x ([])) xs');
+             Prelude.False ->
+              case b1 of {
+               Prelude.True -> app tk (tokenize_helper x0 ((:) x ([])) xs');
+               Prelude.False ->
+                case b2 of {
+                 Prelude.True ->
+                  case b3 of {
+                   Prelude.True ->
+                    app tk (tokenize_helper x0 ((:) x ([])) xs');
+                   Prelude.False ->
+                    case b4 of {
+                     Prelude.True ->
+                      case b5 of {
+                       Prelude.True ->
+                        app tk (tokenize_helper x0 ((:) x ([])) xs');
+                       Prelude.False ->
+                        case b6 of {
+                         Prelude.True ->
+                          app tk (tokenize_helper x0 ((:) x ([])) xs');
+                         Prelude.False ->
+                          app tk ((:) ((:) '(' ([]))
+                            (tokenize_helper Other ([]) xs'))}};
+                     Prelude.False ->
+                      app tk (tokenize_helper x0 ((:) x ([])) xs')}};
+                 Prelude.False ->
+                  app tk (tokenize_helper x0 ((:) x ([])) xs')}}}})
+          x};
+     Alpha ->
+      case classifyChar x of {
+       White ->
+        (\f a -> f (Data.Bits.testBit (Data.Char.ord a) 0)
+              (Data.Bits.testBit (Data.Char.ord a) 1)
+              (Data.Bits.testBit (Data.Char.ord a) 2)
+              (Data.Bits.testBit (Data.Char.ord a) 3)
+              (Data.Bits.testBit (Data.Char.ord a) 4)
+              (Data.Bits.testBit (Data.Char.ord a) 5)
+              (Data.Bits.testBit (Data.Char.ord a) 6)
+              (Data.Bits.testBit (Data.Char.ord a) 7))
+          (\b b0 b1 b2 b3 b4 b5 b6 ->
+          case b of {
+           Prelude.True ->
+            case b0 of {
+             Prelude.True -> app tk (tokenize_helper White ([]) xs');
+             Prelude.False ->
+              case b1 of {
+               Prelude.True -> app tk (tokenize_helper White ([]) xs');
+               Prelude.False ->
+                case b2 of {
+                 Prelude.True ->
+                  case b3 of {
+                   Prelude.True -> app tk (tokenize_helper White ([]) xs');
+                   Prelude.False ->
+                    case b4 of {
+                     Prelude.True ->
+                      case b5 of {
+                       Prelude.True ->
+                        app tk (tokenize_helper White ([]) xs');
+                       Prelude.False ->
+                        case b6 of {
+                         Prelude.True ->
+                          app tk (tokenize_helper White ([]) xs');
+                         Prelude.False ->
+                          app tk ((:) ((:) ')' ([]))
+                            (tokenize_helper Other ([]) xs'))}};
+                     Prelude.False -> app tk (tokenize_helper White ([]) xs')}};
+                 Prelude.False -> app tk (tokenize_helper White ([]) xs')}}};
+           Prelude.False ->
+            case b0 of {
+             Prelude.True -> app tk (tokenize_helper White ([]) xs');
+             Prelude.False ->
+              case b1 of {
+               Prelude.True -> app tk (tokenize_helper White ([]) xs');
+               Prelude.False ->
+                case b2 of {
+                 Prelude.True ->
+                  case b3 of {
+                   Prelude.True -> app tk (tokenize_helper White ([]) xs');
+                   Prelude.False ->
+                    case b4 of {
+                     Prelude.True ->
+                      case b5 of {
+                       Prelude.True ->
+                        app tk (tokenize_helper White ([]) xs');
+                       Prelude.False ->
+                        case b6 of {
+                         Prelude.True ->
+                          app tk (tokenize_helper White ([]) xs');
+                         Prelude.False ->
+                          app tk ((:) ((:) '(' ([]))
+                            (tokenize_helper Other ([]) xs'))}};
+                     Prelude.False -> app tk (tokenize_helper White ([]) xs')}};
+                 Prelude.False -> app tk (tokenize_helper White ([]) xs')}}}})
+          x;
+       Alpha ->
+        (\f a -> f (Data.Bits.testBit (Data.Char.ord a) 0)
+              (Data.Bits.testBit (Data.Char.ord a) 1)
+              (Data.Bits.testBit (Data.Char.ord a) 2)
+              (Data.Bits.testBit (Data.Char.ord a) 3)
+              (Data.Bits.testBit (Data.Char.ord a) 4)
+              (Data.Bits.testBit (Data.Char.ord a) 5)
+              (Data.Bits.testBit (Data.Char.ord a) 6)
+              (Data.Bits.testBit (Data.Char.ord a) 7))
+          (\b b0 b1 b2 b3 b4 b5 b6 ->
+          case b of {
+           Prelude.True ->
+            case b0 of {
+             Prelude.True -> tokenize_helper Alpha ((:) x acc) xs';
+             Prelude.False ->
+              case b1 of {
+               Prelude.True -> tokenize_helper Alpha ((:) x acc) xs';
+               Prelude.False ->
+                case b2 of {
+                 Prelude.True ->
+                  case b3 of {
+                   Prelude.True -> tokenize_helper Alpha ((:) x acc) xs';
+                   Prelude.False ->
+                    case b4 of {
+                     Prelude.True ->
+                      case b5 of {
+                       Prelude.True -> tokenize_helper Alpha ((:) x acc) xs';
+                       Prelude.False ->
+                        case b6 of {
+                         Prelude.True ->
+                          tokenize_helper Alpha ((:) x acc) xs';
+                         Prelude.False ->
+                          app tk ((:) ((:) ')' ([]))
+                            (tokenize_helper Other ([]) xs'))}};
+                     Prelude.False -> tokenize_helper Alpha ((:) x acc) xs'}};
+                 Prelude.False -> tokenize_helper Alpha ((:) x acc) xs'}}};
+           Prelude.False ->
+            case b0 of {
+             Prelude.True -> tokenize_helper Alpha ((:) x acc) xs';
+             Prelude.False ->
+              case b1 of {
+               Prelude.True -> tokenize_helper Alpha ((:) x acc) xs';
+               Prelude.False ->
+                case b2 of {
+                 Prelude.True ->
+                  case b3 of {
+                   Prelude.True -> tokenize_helper Alpha ((:) x acc) xs';
+                   Prelude.False ->
+                    case b4 of {
+                     Prelude.True ->
+                      case b5 of {
+                       Prelude.True -> tokenize_helper Alpha ((:) x acc) xs';
+                       Prelude.False ->
+                        case b6 of {
+                         Prelude.True ->
+                          tokenize_helper Alpha ((:) x acc) xs';
+                         Prelude.False ->
+                          app tk ((:) ((:) '(' ([]))
+                            (tokenize_helper Other ([]) xs'))}};
+                     Prelude.False -> tokenize_helper Alpha ((:) x acc) xs'}};
+                 Prelude.False -> tokenize_helper Alpha ((:) x acc) xs'}}}})
+          x;
+       Digit ->
+        let {tp = Digit} in
+        (\f a -> f (Data.Bits.testBit (Data.Char.ord a) 0)
+              (Data.Bits.testBit (Data.Char.ord a) 1)
+              (Data.Bits.testBit (Data.Char.ord a) 2)
+              (Data.Bits.testBit (Data.Char.ord a) 3)
+              (Data.Bits.testBit (Data.Char.ord a) 4)
+              (Data.Bits.testBit (Data.Char.ord a) 5)
+              (Data.Bits.testBit (Data.Char.ord a) 6)
+              (Data.Bits.testBit (Data.Char.ord a) 7))
+          (\b b0 b1 b2 b3 b4 b5 b6 ->
+          case b of {
+           Prelude.True ->
+            case b0 of {
+             Prelude.True -> app tk (tokenize_helper tp ((:) x ([])) xs');
+             Prelude.False ->
+              case b1 of {
+               Prelude.True -> app tk (tokenize_helper tp ((:) x ([])) xs');
+               Prelude.False ->
+                case b2 of {
+                 Prelude.True ->
+                  case b3 of {
+                   Prelude.True ->
+                    app tk (tokenize_helper tp ((:) x ([])) xs');
+                   Prelude.False ->
+                    case b4 of {
+                     Prelude.True ->
+                      case b5 of {
+                       Prelude.True ->
+                        app tk (tokenize_helper tp ((:) x ([])) xs');
+                       Prelude.False ->
+                        case b6 of {
+                         Prelude.True ->
+                          app tk (tokenize_helper tp ((:) x ([])) xs');
+                         Prelude.False ->
+                          app tk ((:) ((:) ')' ([]))
+                            (tokenize_helper Other ([]) xs'))}};
+                     Prelude.False ->
+                      app tk (tokenize_helper tp ((:) x ([])) xs')}};
+                 Prelude.False ->
+                  app tk (tokenize_helper tp ((:) x ([])) xs')}}};
+           Prelude.False ->
+            case b0 of {
+             Prelude.True -> app tk (tokenize_helper tp ((:) x ([])) xs');
+             Prelude.False ->
+              case b1 of {
+               Prelude.True -> app tk (tokenize_helper tp ((:) x ([])) xs');
+               Prelude.False ->
+                case b2 of {
+                 Prelude.True ->
+                  case b3 of {
+                   Prelude.True ->
+                    app tk (tokenize_helper tp ((:) x ([])) xs');
+                   Prelude.False ->
+                    case b4 of {
+                     Prelude.True ->
+                      case b5 of {
+                       Prelude.True ->
+                        app tk (tokenize_helper tp ((:) x ([])) xs');
+                       Prelude.False ->
+                        case b6 of {
+                         Prelude.True ->
+                          app tk (tokenize_helper tp ((:) x ([])) xs');
+                         Prelude.False ->
+                          app tk ((:) ((:) '(' ([]))
+                            (tokenize_helper Other ([]) xs'))}};
+                     Prelude.False ->
+                      app tk (tokenize_helper tp ((:) x ([])) xs')}};
+                 Prelude.False ->
+                  app tk (tokenize_helper tp ((:) x ([])) xs')}}}})
+          x;
+       Other ->
+        let {tp = Other} in
+        (\f a -> f (Data.Bits.testBit (Data.Char.ord a) 0)
+              (Data.Bits.testBit (Data.Char.ord a) 1)
+              (Data.Bits.testBit (Data.Char.ord a) 2)
+              (Data.Bits.testBit (Data.Char.ord a) 3)
+              (Data.Bits.testBit (Data.Char.ord a) 4)
+              (Data.Bits.testBit (Data.Char.ord a) 5)
+              (Data.Bits.testBit (Data.Char.ord a) 6)
+              (Data.Bits.testBit (Data.Char.ord a) 7))
+          (\b b0 b1 b2 b3 b4 b5 b6 ->
+          case b of {
+           Prelude.True ->
+            case b0 of {
+             Prelude.True -> app tk (tokenize_helper tp ((:) x ([])) xs');
+             Prelude.False ->
+              case b1 of {
+               Prelude.True -> app tk (tokenize_helper tp ((:) x ([])) xs');
+               Prelude.False ->
+                case b2 of {
+                 Prelude.True ->
+                  case b3 of {
+                   Prelude.True ->
+                    app tk (tokenize_helper tp ((:) x ([])) xs');
+                   Prelude.False ->
+                    case b4 of {
+                     Prelude.True ->
+                      case b5 of {
+                       Prelude.True ->
+                        app tk (tokenize_helper tp ((:) x ([])) xs');
+                       Prelude.False ->
+                        case b6 of {
+                         Prelude.True ->
+                          app tk (tokenize_helper tp ((:) x ([])) xs');
+                         Prelude.False ->
+                          app tk ((:) ((:) ')' ([]))
+                            (tokenize_helper Other ([]) xs'))}};
+                     Prelude.False ->
+                      app tk (tokenize_helper tp ((:) x ([])) xs')}};
+                 Prelude.False ->
+                  app tk (tokenize_helper tp ((:) x ([])) xs')}}};
+           Prelude.False ->
+            case b0 of {
+             Prelude.True -> app tk (tokenize_helper tp ((:) x ([])) xs');
+             Prelude.False ->
+              case b1 of {
+               Prelude.True -> app tk (tokenize_helper tp ((:) x ([])) xs');
+               Prelude.False ->
+                case b2 of {
+                 Prelude.True ->
+                  case b3 of {
+                   Prelude.True ->
+                    app tk (tokenize_helper tp ((:) x ([])) xs');
+                   Prelude.False ->
+                    case b4 of {
+                     Prelude.True ->
+                      case b5 of {
+                       Prelude.True ->
+                        app tk (tokenize_helper tp ((:) x ([])) xs');
+                       Prelude.False ->
+                        case b6 of {
+                         Prelude.True ->
+                          app tk (tokenize_helper tp ((:) x ([])) xs');
+                         Prelude.False ->
+                          app tk ((:) ((:) '(' ([]))
+                            (tokenize_helper Other ([]) xs'))}};
+                     Prelude.False ->
+                      app tk (tokenize_helper tp ((:) x ([])) xs')}};
+                 Prelude.False ->
+                  app tk (tokenize_helper tp ((:) x ([])) xs')}}}})
+          x};
+     Digit ->
+      case classifyChar x of {
+       White ->
+        (\f a -> f (Data.Bits.testBit (Data.Char.ord a) 0)
+              (Data.Bits.testBit (Data.Char.ord a) 1)
+              (Data.Bits.testBit (Data.Char.ord a) 2)
+              (Data.Bits.testBit (Data.Char.ord a) 3)
+              (Data.Bits.testBit (Data.Char.ord a) 4)
+              (Data.Bits.testBit (Data.Char.ord a) 5)
+              (Data.Bits.testBit (Data.Char.ord a) 6)
+              (Data.Bits.testBit (Data.Char.ord a) 7))
+          (\b b0 b1 b2 b3 b4 b5 b6 ->
+          case b of {
+           Prelude.True ->
+            case b0 of {
+             Prelude.True -> app tk (tokenize_helper White ([]) xs');
+             Prelude.False ->
+              case b1 of {
+               Prelude.True -> app tk (tokenize_helper White ([]) xs');
+               Prelude.False ->
+                case b2 of {
+                 Prelude.True ->
+                  case b3 of {
+                   Prelude.True -> app tk (tokenize_helper White ([]) xs');
+                   Prelude.False ->
+                    case b4 of {
+                     Prelude.True ->
+                      case b5 of {
+                       Prelude.True ->
+                        app tk (tokenize_helper White ([]) xs');
+                       Prelude.False ->
+                        case b6 of {
+                         Prelude.True ->
+                          app tk (tokenize_helper White ([]) xs');
+                         Prelude.False ->
+                          app tk ((:) ((:) ')' ([]))
+                            (tokenize_helper Other ([]) xs'))}};
+                     Prelude.False -> app tk (tokenize_helper White ([]) xs')}};
+                 Prelude.False -> app tk (tokenize_helper White ([]) xs')}}};
+           Prelude.False ->
+            case b0 of {
+             Prelude.True -> app tk (tokenize_helper White ([]) xs');
+             Prelude.False ->
+              case b1 of {
+               Prelude.True -> app tk (tokenize_helper White ([]) xs');
+               Prelude.False ->
+                case b2 of {
+                 Prelude.True ->
+                  case b3 of {
+                   Prelude.True -> app tk (tokenize_helper White ([]) xs');
+                   Prelude.False ->
+                    case b4 of {
+                     Prelude.True ->
+                      case b5 of {
+                       Prelude.True ->
+                        app tk (tokenize_helper White ([]) xs');
+                       Prelude.False ->
+                        case b6 of {
+                         Prelude.True ->
+                          app tk (tokenize_helper White ([]) xs');
+                         Prelude.False ->
+                          app tk ((:) ((:) '(' ([]))
+                            (tokenize_helper Other ([]) xs'))}};
+                     Prelude.False -> app tk (tokenize_helper White ([]) xs')}};
+                 Prelude.False -> app tk (tokenize_helper White ([]) xs')}}}})
+          x;
+       Alpha ->
+        let {tp = Alpha} in
+        (\f a -> f (Data.Bits.testBit (Data.Char.ord a) 0)
+              (Data.Bits.testBit (Data.Char.ord a) 1)
+              (Data.Bits.testBit (Data.Char.ord a) 2)
+              (Data.Bits.testBit (Data.Char.ord a) 3)
+              (Data.Bits.testBit (Data.Char.ord a) 4)
+              (Data.Bits.testBit (Data.Char.ord a) 5)
+              (Data.Bits.testBit (Data.Char.ord a) 6)
+              (Data.Bits.testBit (Data.Char.ord a) 7))
+          (\b b0 b1 b2 b3 b4 b5 b6 ->
+          case b of {
+           Prelude.True ->
+            case b0 of {
+             Prelude.True -> app tk (tokenize_helper tp ((:) x ([])) xs');
+             Prelude.False ->
+              case b1 of {
+               Prelude.True -> app tk (tokenize_helper tp ((:) x ([])) xs');
+               Prelude.False ->
+                case b2 of {
+                 Prelude.True ->
+                  case b3 of {
+                   Prelude.True ->
+                    app tk (tokenize_helper tp ((:) x ([])) xs');
+                   Prelude.False ->
+                    case b4 of {
+                     Prelude.True ->
+                      case b5 of {
+                       Prelude.True ->
+                        app tk (tokenize_helper tp ((:) x ([])) xs');
+                       Prelude.False ->
+                        case b6 of {
+                         Prelude.True ->
+                          app tk (tokenize_helper tp ((:) x ([])) xs');
+                         Prelude.False ->
+                          app tk ((:) ((:) ')' ([]))
+                            (tokenize_helper Other ([]) xs'))}};
+                     Prelude.False ->
+                      app tk (tokenize_helper tp ((:) x ([])) xs')}};
+                 Prelude.False ->
+                  app tk (tokenize_helper tp ((:) x ([])) xs')}}};
+           Prelude.False ->
+            case b0 of {
+             Prelude.True -> app tk (tokenize_helper tp ((:) x ([])) xs');
+             Prelude.False ->
+              case b1 of {
+               Prelude.True -> app tk (tokenize_helper tp ((:) x ([])) xs');
+               Prelude.False ->
+                case b2 of {
+                 Prelude.True ->
+                  case b3 of {
+                   Prelude.True ->
+                    app tk (tokenize_helper tp ((:) x ([])) xs');
+                   Prelude.False ->
+                    case b4 of {
+                     Prelude.True ->
+                      case b5 of {
+                       Prelude.True ->
+                        app tk (tokenize_helper tp ((:) x ([])) xs');
+                       Prelude.False ->
+                        case b6 of {
+                         Prelude.True ->
+                          app tk (tokenize_helper tp ((:) x ([])) xs');
+                         Prelude.False ->
+                          app tk ((:) ((:) '(' ([]))
+                            (tokenize_helper Other ([]) xs'))}};
+                     Prelude.False ->
+                      app tk (tokenize_helper tp ((:) x ([])) xs')}};
+                 Prelude.False ->
+                  app tk (tokenize_helper tp ((:) x ([])) xs')}}}})
+          x;
+       Digit ->
+        (\f a -> f (Data.Bits.testBit (Data.Char.ord a) 0)
+              (Data.Bits.testBit (Data.Char.ord a) 1)
+              (Data.Bits.testBit (Data.Char.ord a) 2)
+              (Data.Bits.testBit (Data.Char.ord a) 3)
+              (Data.Bits.testBit (Data.Char.ord a) 4)
+              (Data.Bits.testBit (Data.Char.ord a) 5)
+              (Data.Bits.testBit (Data.Char.ord a) 6)
+              (Data.Bits.testBit (Data.Char.ord a) 7))
+          (\b b0 b1 b2 b3 b4 b5 b6 ->
+          case b of {
+           Prelude.True ->
+            case b0 of {
+             Prelude.True -> tokenize_helper Digit ((:) x acc) xs';
+             Prelude.False ->
+              case b1 of {
+               Prelude.True -> tokenize_helper Digit ((:) x acc) xs';
+               Prelude.False ->
+                case b2 of {
+                 Prelude.True ->
+                  case b3 of {
+                   Prelude.True -> tokenize_helper Digit ((:) x acc) xs';
+                   Prelude.False ->
+                    case b4 of {
+                     Prelude.True ->
+                      case b5 of {
+                       Prelude.True -> tokenize_helper Digit ((:) x acc) xs';
+                       Prelude.False ->
+                        case b6 of {
+                         Prelude.True ->
+                          tokenize_helper Digit ((:) x acc) xs';
+                         Prelude.False ->
+                          app tk ((:) ((:) ')' ([]))
+                            (tokenize_helper Other ([]) xs'))}};
+                     Prelude.False -> tokenize_helper Digit ((:) x acc) xs'}};
+                 Prelude.False -> tokenize_helper Digit ((:) x acc) xs'}}};
+           Prelude.False ->
+            case b0 of {
+             Prelude.True -> tokenize_helper Digit ((:) x acc) xs';
+             Prelude.False ->
+              case b1 of {
+               Prelude.True -> tokenize_helper Digit ((:) x acc) xs';
+               Prelude.False ->
+                case b2 of {
+                 Prelude.True ->
+                  case b3 of {
+                   Prelude.True -> tokenize_helper Digit ((:) x acc) xs';
+                   Prelude.False ->
+                    case b4 of {
+                     Prelude.True ->
+                      case b5 of {
+                       Prelude.True -> tokenize_helper Digit ((:) x acc) xs';
+                       Prelude.False ->
+                        case b6 of {
+                         Prelude.True ->
+                          tokenize_helper Digit ((:) x acc) xs';
+                         Prelude.False ->
+                          app tk ((:) ((:) '(' ([]))
+                            (tokenize_helper Other ([]) xs'))}};
+                     Prelude.False -> tokenize_helper Digit ((:) x acc) xs'}};
+                 Prelude.False -> tokenize_helper Digit ((:) x acc) xs'}}}})
+          x;
+       Other ->
+        let {tp = Other} in
+        (\f a -> f (Data.Bits.testBit (Data.Char.ord a) 0)
+              (Data.Bits.testBit (Data.Char.ord a) 1)
+              (Data.Bits.testBit (Data.Char.ord a) 2)
+              (Data.Bits.testBit (Data.Char.ord a) 3)
+              (Data.Bits.testBit (Data.Char.ord a) 4)
+              (Data.Bits.testBit (Data.Char.ord a) 5)
+              (Data.Bits.testBit (Data.Char.ord a) 6)
+              (Data.Bits.testBit (Data.Char.ord a) 7))
+          (\b b0 b1 b2 b3 b4 b5 b6 ->
+          case b of {
+           Prelude.True ->
+            case b0 of {
+             Prelude.True -> app tk (tokenize_helper tp ((:) x ([])) xs');
+             Prelude.False ->
+              case b1 of {
+               Prelude.True -> app tk (tokenize_helper tp ((:) x ([])) xs');
+               Prelude.False ->
+                case b2 of {
+                 Prelude.True ->
+                  case b3 of {
+                   Prelude.True ->
+                    app tk (tokenize_helper tp ((:) x ([])) xs');
+                   Prelude.False ->
+                    case b4 of {
+                     Prelude.True ->
+                      case b5 of {
+                       Prelude.True ->
+                        app tk (tokenize_helper tp ((:) x ([])) xs');
+                       Prelude.False ->
+                        case b6 of {
+                         Prelude.True ->
+                          app tk (tokenize_helper tp ((:) x ([])) xs');
+                         Prelude.False ->
+                          app tk ((:) ((:) ')' ([]))
+                            (tokenize_helper Other ([]) xs'))}};
+                     Prelude.False ->
+                      app tk (tokenize_helper tp ((:) x ([])) xs')}};
+                 Prelude.False ->
+                  app tk (tokenize_helper tp ((:) x ([])) xs')}}};
+           Prelude.False ->
+            case b0 of {
+             Prelude.True -> app tk (tokenize_helper tp ((:) x ([])) xs');
+             Prelude.False ->
+              case b1 of {
+               Prelude.True -> app tk (tokenize_helper tp ((:) x ([])) xs');
+               Prelude.False ->
+                case b2 of {
+                 Prelude.True ->
+                  case b3 of {
+                   Prelude.True ->
+                    app tk (tokenize_helper tp ((:) x ([])) xs');
+                   Prelude.False ->
+                    case b4 of {
+                     Prelude.True ->
+                      case b5 of {
+                       Prelude.True ->
+                        app tk (tokenize_helper tp ((:) x ([])) xs');
+                       Prelude.False ->
+                        case b6 of {
+                         Prelude.True ->
+                          app tk (tokenize_helper tp ((:) x ([])) xs');
+                         Prelude.False ->
+                          app tk ((:) ((:) '(' ([]))
+                            (tokenize_helper Other ([]) xs'))}};
+                     Prelude.False ->
+                      app tk (tokenize_helper tp ((:) x ([])) xs')}};
+                 Prelude.False ->
+                  app tk (tokenize_helper tp ((:) x ([])) xs')}}}})
+          x};
+     Other ->
+      case classifyChar x of {
+       White ->
+        (\f a -> f (Data.Bits.testBit (Data.Char.ord a) 0)
+              (Data.Bits.testBit (Data.Char.ord a) 1)
+              (Data.Bits.testBit (Data.Char.ord a) 2)
+              (Data.Bits.testBit (Data.Char.ord a) 3)
+              (Data.Bits.testBit (Data.Char.ord a) 4)
+              (Data.Bits.testBit (Data.Char.ord a) 5)
+              (Data.Bits.testBit (Data.Char.ord a) 6)
+              (Data.Bits.testBit (Data.Char.ord a) 7))
+          (\b b0 b1 b2 b3 b4 b5 b6 ->
+          case b of {
+           Prelude.True ->
+            case b0 of {
+             Prelude.True -> app tk (tokenize_helper White ([]) xs');
+             Prelude.False ->
+              case b1 of {
+               Prelude.True -> app tk (tokenize_helper White ([]) xs');
+               Prelude.False ->
+                case b2 of {
+                 Prelude.True ->
+                  case b3 of {
+                   Prelude.True -> app tk (tokenize_helper White ([]) xs');
+                   Prelude.False ->
+                    case b4 of {
+                     Prelude.True ->
+                      case b5 of {
+                       Prelude.True ->
+                        app tk (tokenize_helper White ([]) xs');
+                       Prelude.False ->
+                        case b6 of {
+                         Prelude.True ->
+                          app tk (tokenize_helper White ([]) xs');
+                         Prelude.False ->
+                          app tk ((:) ((:) ')' ([]))
+                            (tokenize_helper Other ([]) xs'))}};
+                     Prelude.False -> app tk (tokenize_helper White ([]) xs')}};
+                 Prelude.False -> app tk (tokenize_helper White ([]) xs')}}};
+           Prelude.False ->
+            case b0 of {
+             Prelude.True -> app tk (tokenize_helper White ([]) xs');
+             Prelude.False ->
+              case b1 of {
+               Prelude.True -> app tk (tokenize_helper White ([]) xs');
+               Prelude.False ->
+                case b2 of {
+                 Prelude.True ->
+                  case b3 of {
+                   Prelude.True -> app tk (tokenize_helper White ([]) xs');
+                   Prelude.False ->
+                    case b4 of {
+                     Prelude.True ->
+                      case b5 of {
+                       Prelude.True ->
+                        app tk (tokenize_helper White ([]) xs');
+                       Prelude.False ->
+                        case b6 of {
+                         Prelude.True ->
+                          app tk (tokenize_helper White ([]) xs');
+                         Prelude.False ->
+                          app tk ((:) ((:) '(' ([]))
+                            (tokenize_helper Other ([]) xs'))}};
+                     Prelude.False -> app tk (tokenize_helper White ([]) xs')}};
+                 Prelude.False -> app tk (tokenize_helper White ([]) xs')}}}})
+          x;
+       Other ->
+        (\f a -> f (Data.Bits.testBit (Data.Char.ord a) 0)
+              (Data.Bits.testBit (Data.Char.ord a) 1)
+              (Data.Bits.testBit (Data.Char.ord a) 2)
+              (Data.Bits.testBit (Data.Char.ord a) 3)
+              (Data.Bits.testBit (Data.Char.ord a) 4)
+              (Data.Bits.testBit (Data.Char.ord a) 5)
+              (Data.Bits.testBit (Data.Char.ord a) 6)
+              (Data.Bits.testBit (Data.Char.ord a) 7))
+          (\b b0 b1 b2 b3 b4 b5 b6 ->
+          case b of {
+           Prelude.True ->
+            case b0 of {
+             Prelude.True -> tokenize_helper Other ((:) x acc) xs';
+             Prelude.False ->
+              case b1 of {
+               Prelude.True -> tokenize_helper Other ((:) x acc) xs';
+               Prelude.False ->
+                case b2 of {
+                 Prelude.True ->
+                  case b3 of {
+                   Prelude.True -> tokenize_helper Other ((:) x acc) xs';
+                   Prelude.False ->
+                    case b4 of {
+                     Prelude.True ->
+                      case b5 of {
+                       Prelude.True -> tokenize_helper Other ((:) x acc) xs';
+                       Prelude.False ->
+                        case b6 of {
+                         Prelude.True ->
+                          tokenize_helper Other ((:) x acc) xs';
+                         Prelude.False ->
+                          app tk ((:) ((:) ')' ([]))
+                            (tokenize_helper Other ([]) xs'))}};
+                     Prelude.False -> tokenize_helper Other ((:) x acc) xs'}};
+                 Prelude.False -> tokenize_helper Other ((:) x acc) xs'}}};
+           Prelude.False ->
+            case b0 of {
+             Prelude.True -> tokenize_helper Other ((:) x acc) xs';
+             Prelude.False ->
+              case b1 of {
+               Prelude.True -> tokenize_helper Other ((:) x acc) xs';
+               Prelude.False ->
+                case b2 of {
+                 Prelude.True ->
+                  case b3 of {
+                   Prelude.True -> tokenize_helper Other ((:) x acc) xs';
+                   Prelude.False ->
+                    case b4 of {
+                     Prelude.True ->
+                      case b5 of {
+                       Prelude.True -> tokenize_helper Other ((:) x acc) xs';
+                       Prelude.False ->
+                        case b6 of {
+                         Prelude.True ->
+                          tokenize_helper Other ((:) x acc) xs';
+                         Prelude.False ->
+                          app tk ((:) ((:) '(' ([]))
+                            (tokenize_helper Other ([]) xs'))}};
+                     Prelude.False -> tokenize_helper Other ((:) x acc) xs'}};
+                 Prelude.False -> tokenize_helper Other ((:) x acc) xs'}}}})
+          x;
+       x0 ->
+        (\f a -> f (Data.Bits.testBit (Data.Char.ord a) 0)
+              (Data.Bits.testBit (Data.Char.ord a) 1)
+              (Data.Bits.testBit (Data.Char.ord a) 2)
+              (Data.Bits.testBit (Data.Char.ord a) 3)
+              (Data.Bits.testBit (Data.Char.ord a) 4)
+              (Data.Bits.testBit (Data.Char.ord a) 5)
+              (Data.Bits.testBit (Data.Char.ord a) 6)
+              (Data.Bits.testBit (Data.Char.ord a) 7))
+          (\b b0 b1 b2 b3 b4 b5 b6 ->
+          case b of {
+           Prelude.True ->
+            case b0 of {
+             Prelude.True -> app tk (tokenize_helper x0 ((:) x ([])) xs');
+             Prelude.False ->
+              case b1 of {
+               Prelude.True -> app tk (tokenize_helper x0 ((:) x ([])) xs');
+               Prelude.False ->
+                case b2 of {
+                 Prelude.True ->
+                  case b3 of {
+                   Prelude.True ->
+                    app tk (tokenize_helper x0 ((:) x ([])) xs');
+                   Prelude.False ->
+                    case b4 of {
+                     Prelude.True ->
+                      case b5 of {
+                       Prelude.True ->
+                        app tk (tokenize_helper x0 ((:) x ([])) xs');
+                       Prelude.False ->
+                        case b6 of {
+                         Prelude.True ->
+                          app tk (tokenize_helper x0 ((:) x ([])) xs');
+                         Prelude.False ->
+                          app tk ((:) ((:) ')' ([]))
+                            (tokenize_helper Other ([]) xs'))}};
+                     Prelude.False ->
+                      app tk (tokenize_helper x0 ((:) x ([])) xs')}};
+                 Prelude.False ->
+                  app tk (tokenize_helper x0 ((:) x ([])) xs')}}};
+           Prelude.False ->
+            case b0 of {
+             Prelude.True -> app tk (tokenize_helper x0 ((:) x ([])) xs');
+             Prelude.False ->
+              case b1 of {
+               Prelude.True -> app tk (tokenize_helper x0 ((:) x ([])) xs');
+               Prelude.False ->
+                case b2 of {
+                 Prelude.True ->
+                  case b3 of {
+                   Prelude.True ->
+                    app tk (tokenize_helper x0 ((:) x ([])) xs');
+                   Prelude.False ->
+                    case b4 of {
+                     Prelude.True ->
+                      case b5 of {
+                       Prelude.True ->
+                        app tk (tokenize_helper x0 ((:) x ([])) xs');
+                       Prelude.False ->
+                        case b6 of {
+                         Prelude.True ->
+                          app tk (tokenize_helper x0 ((:) x ([])) xs');
+                         Prelude.False ->
+                          app tk ((:) ((:) '(' ([]))
+                            (tokenize_helper Other ([]) xs'))}};
+                     Prelude.False ->
+                      app tk (tokenize_helper x0 ((:) x ([])) xs')}};
+                 Prelude.False ->
+                  app tk (tokenize_helper x0 ((:) x ([])) xs')}}}})
+          x}}}
+
+tokenize :: Prelude.String -> ([]) Prelude.String
+tokenize s =
+  map string_of_list (tokenize_helper White ([]) (list_of_string s))
+
+type Parser a =
+  (([]) Prelude.String) -> Prelude.Either (([]) Prelude.String)
+  ((,) a (([]) Prelude.String))
+  -- singleton inductive, whose constructor was Parser
+  
+pure :: a1 -> Parser a1
+pure x input =
+  Prelude.Right ((,) x input)
+
+bind :: (Parser a1) -> (a1 -> Parser a2) -> Parser a2
+bind p f input =
+  case p input of {
+   Prelude.Left err -> Prelude.Left err;
+   Prelude.Right p0 -> case p0 of {
+                        (,) result rest -> f result rest}}
+
+bind_discard_L :: (Parser a1) -> (Parser a2) -> Parser a2
+bind_discard_L p p' input =
+  case p input of {
+   Prelude.Left err -> Prelude.Left err;
+   Prelude.Right p0 -> case p0 of {
+                        (,) _ rest -> p' rest}}
+
+alternative :: (Parser a1) -> (Parser a1) -> Parser a1
+alternative p1 p2 input =
+  case p1 input of {
+   Prelude.Left err1 ->
+    case p2 input of {
+     Prelude.Left err2 -> Prelude.Left (app err1 err2);
+     Prelude.Right p -> Prelude.Right p};
+   Prelude.Right p -> Prelude.Right p}
+
+fail_parser :: Parser a1
+fail_parser _ =
+  Prelude.Left ((:) "Failed to parse." ([]))
+
+parse_map :: (a1 -> a2) -> (Parser a1) -> Parser a2
+parse_map f p input =
+  case p input of {
+   Prelude.Left err -> Prelude.Left err;
+   Prelude.Right p0 ->
+    case p0 of {
+     (,) result rest -> Prelude.Right ((,) (f result) rest)}}
+
+parse :: (Parser a1) -> Prelude.String -> Prelude.Either
+         (([]) Prelude.String) ((,) a1 (([]) Prelude.String))
+parse p input =
+  p (tokenize input)
+
+parse_nat :: Parser Prelude.Integer
+parse_nat input =
+  case input of {
+   ([]) -> Prelude.Left ((:) "Nothing to parse." ([]));
+   (:) h t ->
+    case string_to_nat h of {
+     Prelude.Just n -> Prelude.Right ((,) n t);
+     Prelude.Nothing -> Prelude.Left ((:)
+      (append "Not a valid number: "
+        (append "'"
+          (append h
+            (append "', expected a number at '"
+              (append (concat_string_list ((:) h ((:) " " t))) "'.")))))
+      ([]))}}
+
+parse_var_name :: Parser Prelude.String
+parse_var_name input =
+  case input of {
+   ([]) -> Prelude.Left ((:) "Nothing to parse." ([]));
+   (:) h t ->
+    case forallb isLowerAlpha (list_of_string h) of {
+     Prelude.True -> Prelude.Right ((,) h t);
+     Prelude.False -> Prelude.Left ((:)
+      (append "Not a valid variable string: "
+        (append "'"
+          (append h
+            (append "', expected a string at '"
+              (append (concat_string_list ((:) h ((:) " " t))) "'.")))))
+      ([]))}}
+
+parse_keyword :: Prelude.String -> Parser Prelude.String
+parse_keyword keyword input =
+  case input of {
+   ([]) -> Prelude.Left ((:) "Nothing to parse." ([]));
+   (:) h t ->
+    case ((Prelude.==) :: Prelude.String -> Prelude.String -> Prelude.Bool)
+           keyword h of {
+     Prelude.True -> Prelude.Right ((,) keyword t);
+     Prelude.False -> Prelude.Left ((:)
+      (append "Not a valid keyword: "
+        (append "'"
+          (append h
+            (append "', expected '"
+              (append keyword
+                (append "' at '"
+                  (append (concat_string_list ((:) h ((:) " " t))) "'.")))))))
+      ([]))}}
+
+parse_Var :: Parser Expr
+parse_Var =
+  bind parse_var_name (\x -> pure (Var x))
+
+parse_Add :: Parser (Expr -> Expr -> Expr)
+parse_Add =
+  bind_discard_L (parse_keyword "+") (pure (\x x0 -> Add x x0))
+
+parse_Sub :: Parser (Expr -> Expr -> Expr)
+parse_Sub =
+  bind_discard_L (parse_keyword "-") (pure (\x x0 -> Sub x x0))
+
+parse_Mul :: Parser (Expr -> Expr -> Expr)
+parse_Mul =
+  bind_discard_L (parse_keyword "*") (pure (\x x0 -> Mul x x0))
+
+parse_Lambda :: (Parser Expr) -> Parser Expr
+parse_Lambda p =
+  bind_discard_L (parse_keyword "\\")
+    (bind parse_var_name (\x ->
+      bind_discard_L (parse_keyword "->") (bind p (\f -> pure (Lambda x f)))))
+
+parse_Apply :: Parser (Expr -> Expr -> Expr)
+parse_Apply =
+  bind_discard_L (parse_keyword ".") (pure (\x x0 -> Apply x x0))
+
+parse_Cond :: (Parser Expr) -> Parser Expr
+parse_Cond p =
+  bind_discard_L (parse_keyword "If")
+    (bind p (\e1 ->
+      bind_discard_L (parse_keyword "Then")
+        (bind p (\e2 ->
+          bind_discard_L (parse_keyword "Else")
+            (bind p (\e3 -> pure (Cond e1 e2 e3)))))))
+
+parse_Bool :: Parser Expr
+parse_Bool =
+  bind (alternative (parse_keyword "True") (parse_keyword "False")) (\p ->
+    case p of {
+     ([]) -> fail_parser;
+     (:) a s ->
+      (\f a -> f (Data.Bits.testBit (Data.Char.ord a) 0)
+              (Data.Bits.testBit (Data.Char.ord a) 1)
+              (Data.Bits.testBit (Data.Char.ord a) 2)
+              (Data.Bits.testBit (Data.Char.ord a) 3)
+              (Data.Bits.testBit (Data.Char.ord a) 4)
+              (Data.Bits.testBit (Data.Char.ord a) 5)
+              (Data.Bits.testBit (Data.Char.ord a) 6)
+              (Data.Bits.testBit (Data.Char.ord a) 7))
+        (\b b0 b1 b2 b3 b4 b5 b6 ->
+        case b of {
+         Prelude.True -> fail_parser;
+         Prelude.False ->
+          case b0 of {
+           Prelude.True ->
+            case b1 of {
+             Prelude.True ->
+              case b2 of {
+               Prelude.True -> fail_parser;
+               Prelude.False ->
+                case b3 of {
+                 Prelude.True -> fail_parser;
+                 Prelude.False ->
+                  case b4 of {
+                   Prelude.True -> fail_parser;
+                   Prelude.False ->
+                    case b5 of {
+                     Prelude.True ->
+                      case b6 of {
+                       Prelude.True -> fail_parser;
+                       Prelude.False ->
+                        case s of {
+                         ([]) -> fail_parser;
+                         (:) a0 s0 ->
+                          (\f a -> f (Data.Bits.testBit (Data.Char.ord a) 0)
+              (Data.Bits.testBit (Data.Char.ord a) 1)
+              (Data.Bits.testBit (Data.Char.ord a) 2)
+              (Data.Bits.testBit (Data.Char.ord a) 3)
+              (Data.Bits.testBit (Data.Char.ord a) 4)
+              (Data.Bits.testBit (Data.Char.ord a) 5)
+              (Data.Bits.testBit (Data.Char.ord a) 6)
+              (Data.Bits.testBit (Data.Char.ord a) 7))
+                            (\b7 b8 b9 b10 b11 b12 b13 b14 ->
+                            case b7 of {
+                             Prelude.True ->
+                              case b8 of {
+                               Prelude.True -> fail_parser;
+                               Prelude.False ->
+                                case b9 of {
+                                 Prelude.True -> fail_parser;
+                                 Prelude.False ->
+                                  case b10 of {
+                                   Prelude.True -> fail_parser;
+                                   Prelude.False ->
+                                    case b11 of {
+                                     Prelude.True -> fail_parser;
+                                     Prelude.False ->
+                                      case b12 of {
+                                       Prelude.True ->
+                                        case b13 of {
+                                         Prelude.True ->
+                                          case b14 of {
+                                           Prelude.True -> fail_parser;
+                                           Prelude.False ->
+                                            case s0 of {
+                                             ([]) -> fail_parser;
+                                             (:) a1 s1 ->
+                                              (\f a -> f (Data.Bits.testBit (Data.Char.ord a) 0)
+              (Data.Bits.testBit (Data.Char.ord a) 1)
+              (Data.Bits.testBit (Data.Char.ord a) 2)
+              (Data.Bits.testBit (Data.Char.ord a) 3)
+              (Data.Bits.testBit (Data.Char.ord a) 4)
+              (Data.Bits.testBit (Data.Char.ord a) 5)
+              (Data.Bits.testBit (Data.Char.ord a) 6)
+              (Data.Bits.testBit (Data.Char.ord a) 7))
+                                                (\b15 b16 b17 b18 b19 b20 b21 b22 ->
+                                                case b15 of {
+                                                 Prelude.True -> fail_parser;
+                                                 Prelude.False ->
+                                                  case b16 of {
+                                                   Prelude.True ->
+                                                    fail_parser;
+                                                   Prelude.False ->
+                                                    case b17 of {
+                                                     Prelude.True ->
+                                                      case b18 of {
+                                                       Prelude.True ->
+                                                        case b19 of {
+                                                         Prelude.True ->
+                                                          fail_parser;
+                                                         Prelude.False ->
+                                                          case b20 of {
+                                                           Prelude.True ->
+                                                            case b21 of {
+                                                             Prelude.True ->
+                                                              case b22 of {
+                                                               Prelude.True ->
+                                                                fail_parser;
+                                                               Prelude.False ->
+                                                                case s1 of {
+                                                                 ([]) ->
+                                                                  fail_parser;
+                                                                 (:) a2 s2 ->
+                                                                  (\f a -> f (Data.Bits.testBit (Data.Char.ord a) 0)
+              (Data.Bits.testBit (Data.Char.ord a) 1)
+              (Data.Bits.testBit (Data.Char.ord a) 2)
+              (Data.Bits.testBit (Data.Char.ord a) 3)
+              (Data.Bits.testBit (Data.Char.ord a) 4)
+              (Data.Bits.testBit (Data.Char.ord a) 5)
+              (Data.Bits.testBit (Data.Char.ord a) 6)
+              (Data.Bits.testBit (Data.Char.ord a) 7))
+                                                                    (\b23 b24 b25 b26 b27 b28 b29 b30 ->
+                                                                    case b23 of {
+                                                                     Prelude.True ->
+                                                                    case b24 of {
+                                                                     Prelude.True ->
+                                                                    case b25 of {
+                                                                     Prelude.True ->
+                                                                    fail_parser;
+                                                                     Prelude.False ->
+                                                                    case b26 of {
+                                                                     Prelude.True ->
+                                                                    fail_parser;
+                                                                     Prelude.False ->
+                                                                    case b27 of {
+                                                                     Prelude.True ->
+                                                                    case b28 of {
+                                                                     Prelude.True ->
+                                                                    case b29 of {
+                                                                     Prelude.True ->
+                                                                    case b30 of {
+                                                                     Prelude.True ->
+                                                                    fail_parser;
+                                                                     Prelude.False ->
+                                                                    case s2 of {
+                                                                     ([]) ->
+                                                                    fail_parser;
+                                                                     (:) a3
+                                                                    s3 ->
+                                                                    (\f a -> f (Data.Bits.testBit (Data.Char.ord a) 0)
+              (Data.Bits.testBit (Data.Char.ord a) 1)
+              (Data.Bits.testBit (Data.Char.ord a) 2)
+              (Data.Bits.testBit (Data.Char.ord a) 3)
+              (Data.Bits.testBit (Data.Char.ord a) 4)
+              (Data.Bits.testBit (Data.Char.ord a) 5)
+              (Data.Bits.testBit (Data.Char.ord a) 6)
+              (Data.Bits.testBit (Data.Char.ord a) 7))
+                                                                    (\b31 b32 b33 b34 b35 b36 b37 b38 ->
+                                                                    case b31 of {
+                                                                     Prelude.True ->
+                                                                    case b32 of {
+                                                                     Prelude.True ->
+                                                                    fail_parser;
+                                                                     Prelude.False ->
+                                                                    case b33 of {
+                                                                     Prelude.True ->
+                                                                    case b34 of {
+                                                                     Prelude.True ->
+                                                                    fail_parser;
+                                                                     Prelude.False ->
+                                                                    case b35 of {
+                                                                     Prelude.True ->
+                                                                    fail_parser;
+                                                                     Prelude.False ->
+                                                                    case b36 of {
+                                                                     Prelude.True ->
+                                                                    case b37 of {
+                                                                     Prelude.True ->
+                                                                    case b38 of {
+                                                                     Prelude.True ->
+                                                                    fail_parser;
+                                                                     Prelude.False ->
+                                                                    case s3 of {
+                                                                     ([]) ->
+                                                                    pure
+                                                                    (Bool
+                                                                    Prelude.False);
+                                                                     (:) _
+                                                                    _ ->
+                                                                    fail_parser}};
+                                                                     Prelude.False ->
+                                                                    fail_parser};
+                                                                     Prelude.False ->
+                                                                    fail_parser}}};
+                                                                     Prelude.False ->
+                                                                    fail_parser}};
+                                                                     Prelude.False ->
+                                                                    fail_parser})
+                                                                    a3}};
+                                                                     Prelude.False ->
+                                                                    fail_parser};
+                                                                     Prelude.False ->
+                                                                    fail_parser};
+                                                                     Prelude.False ->
+                                                                    fail_parser}}};
+                                                                     Prelude.False ->
+                                                                    fail_parser};
+                                                                     Prelude.False ->
+                                                                    fail_parser})
+                                                                    a2}};
+                                                             Prelude.False ->
+                                                              fail_parser};
+                                                           Prelude.False ->
+                                                            fail_parser}};
+                                                       Prelude.False ->
+                                                        fail_parser};
+                                                     Prelude.False ->
+                                                      fail_parser}}})
+                                                a1}};
+                                         Prelude.False -> fail_parser};
+                                       Prelude.False -> fail_parser}}}}};
+                             Prelude.False -> fail_parser})
+                            a0}};
+                     Prelude.False -> fail_parser}}}};
+             Prelude.False -> fail_parser};
+           Prelude.False ->
+            case b1 of {
+             Prelude.True ->
+              case b2 of {
+               Prelude.True -> fail_parser;
+               Prelude.False ->
+                case b3 of {
+                 Prelude.True ->
+                  case b4 of {
+                   Prelude.True -> fail_parser;
+                   Prelude.False ->
+                    case b5 of {
+                     Prelude.True ->
+                      case b6 of {
+                       Prelude.True -> fail_parser;
+                       Prelude.False ->
+                        case s of {
+                         ([]) -> fail_parser;
+                         (:) a0 s0 ->
+                          (\f a -> f (Data.Bits.testBit (Data.Char.ord a) 0)
+              (Data.Bits.testBit (Data.Char.ord a) 1)
+              (Data.Bits.testBit (Data.Char.ord a) 2)
+              (Data.Bits.testBit (Data.Char.ord a) 3)
+              (Data.Bits.testBit (Data.Char.ord a) 4)
+              (Data.Bits.testBit (Data.Char.ord a) 5)
+              (Data.Bits.testBit (Data.Char.ord a) 6)
+              (Data.Bits.testBit (Data.Char.ord a) 7))
+                            (\b7 b8 b9 b10 b11 b12 b13 b14 ->
+                            case b7 of {
+                             Prelude.True -> fail_parser;
+                             Prelude.False ->
+                              case b8 of {
+                               Prelude.True ->
+                                case b9 of {
+                                 Prelude.True -> fail_parser;
+                                 Prelude.False ->
+                                  case b10 of {
+                                   Prelude.True -> fail_parser;
+                                   Prelude.False ->
+                                    case b11 of {
+                                     Prelude.True ->
+                                      case b12 of {
+                                       Prelude.True ->
+                                        case b13 of {
+                                         Prelude.True ->
+                                          case b14 of {
+                                           Prelude.True -> fail_parser;
+                                           Prelude.False ->
+                                            case s0 of {
+                                             ([]) -> fail_parser;
+                                             (:) a1 s1 ->
+                                              (\f a -> f (Data.Bits.testBit (Data.Char.ord a) 0)
+              (Data.Bits.testBit (Data.Char.ord a) 1)
+              (Data.Bits.testBit (Data.Char.ord a) 2)
+              (Data.Bits.testBit (Data.Char.ord a) 3)
+              (Data.Bits.testBit (Data.Char.ord a) 4)
+              (Data.Bits.testBit (Data.Char.ord a) 5)
+              (Data.Bits.testBit (Data.Char.ord a) 6)
+              (Data.Bits.testBit (Data.Char.ord a) 7))
+                                                (\b15 b16 b17 b18 b19 b20 b21 b22 ->
+                                                case b15 of {
+                                                 Prelude.True ->
+                                                  case b16 of {
+                                                   Prelude.True ->
+                                                    fail_parser;
+                                                   Prelude.False ->
+                                                    case b17 of {
+                                                     Prelude.True ->
+                                                      case b18 of {
+                                                       Prelude.True ->
+                                                        fail_parser;
+                                                       Prelude.False ->
+                                                        case b19 of {
+                                                         Prelude.True ->
+                                                          case b20 of {
+                                                           Prelude.True ->
+                                                            case b21 of {
+                                                             Prelude.True ->
+                                                              case b22 of {
+                                                               Prelude.True ->
+                                                                fail_parser;
+                                                               Prelude.False ->
+                                                                case s1 of {
+                                                                 ([]) ->
+                                                                  fail_parser;
+                                                                 (:) a2 s2 ->
+                                                                  (\f a -> f (Data.Bits.testBit (Data.Char.ord a) 0)
+              (Data.Bits.testBit (Data.Char.ord a) 1)
+              (Data.Bits.testBit (Data.Char.ord a) 2)
+              (Data.Bits.testBit (Data.Char.ord a) 3)
+              (Data.Bits.testBit (Data.Char.ord a) 4)
+              (Data.Bits.testBit (Data.Char.ord a) 5)
+              (Data.Bits.testBit (Data.Char.ord a) 6)
+              (Data.Bits.testBit (Data.Char.ord a) 7))
+                                                                    (\b23 b24 b25 b26 b27 b28 b29 b30 ->
+                                                                    case b23 of {
+                                                                     Prelude.True ->
+                                                                    case b24 of {
+                                                                     Prelude.True ->
+                                                                    fail_parser;
+                                                                     Prelude.False ->
+                                                                    case b25 of {
+                                                                     Prelude.True ->
+                                                                    case b26 of {
+                                                                     Prelude.True ->
+                                                                    fail_parser;
+                                                                     Prelude.False ->
+                                                                    case b27 of {
+                                                                     Prelude.True ->
+                                                                    fail_parser;
+                                                                     Prelude.False ->
+                                                                    case b28 of {
+                                                                     Prelude.True ->
+                                                                    case b29 of {
+                                                                     Prelude.True ->
+                                                                    case b30 of {
+                                                                     Prelude.True ->
+                                                                    fail_parser;
+                                                                     Prelude.False ->
+                                                                    case s2 of {
+                                                                     ([]) ->
+                                                                    pure
+                                                                    (Bool
+                                                                    Prelude.True);
+                                                                     (:) _
+                                                                    _ ->
+                                                                    fail_parser}};
+                                                                     Prelude.False ->
+                                                                    fail_parser};
+                                                                     Prelude.False ->
+                                                                    fail_parser}}};
+                                                                     Prelude.False ->
+                                                                    fail_parser}};
+                                                                     Prelude.False ->
+                                                                    fail_parser})
+                                                                    a2}};
+                                                             Prelude.False ->
+                                                              fail_parser};
+                                                           Prelude.False ->
+                                                            fail_parser};
+                                                         Prelude.False ->
+                                                          fail_parser}};
+                                                     Prelude.False ->
+                                                      fail_parser}};
+                                                 Prelude.False -> fail_parser})
+                                                a1}};
+                                         Prelude.False -> fail_parser};
+                                       Prelude.False -> fail_parser};
+                                     Prelude.False -> fail_parser}}};
+                               Prelude.False -> fail_parser}})
+                            a0}};
+                     Prelude.False -> fail_parser}};
+                 Prelude.False -> fail_parser}};
+             Prelude.False -> fail_parser}}})
+        a})
+
+parse_Nat :: Parser Expr
+parse_Nat =
+  parse_map (\x -> Nat x) parse_nat
+
+parse_Eq :: (Parser Expr) -> Parser Expr
+parse_Eq p =
+  bind_discard_L (parse_keyword "{")
+    (bind p (\a1 ->
+      bind_discard_L (parse_keyword "==")
+        (bind p (\a2 ->
+          bind_discard_L (parse_keyword "}") (pure (Eq a1 a2))))))
+
+parse_And :: Parser (Expr -> Expr -> Expr)
+parse_And =
+  bind_discard_L (parse_keyword "&&") (pure (\x x0 -> And x x0))
+
+parse_Let :: (Parser Expr) -> Parser Expr
+parse_Let p =
+  bind_discard_L (parse_keyword "Let")
+    (bind parse_var_name (\x ->
+      bind_discard_L (parse_keyword ":=")
+        (bind p (\f ->
+          bind_discard_L (parse_keyword "In")
+            (bind p (\f' -> pure (Let x f f')))))))
+
+parse_Expr :: Prelude.Integer -> Parser Expr
+parse_Expr n =
+  (\fO fS n -> if n Prelude.== 0 then fO () else fS (n Prelude.- 1))
+    (\_ -> fail_parser)
+    (\n' ->
+    let {
+     parse_Sub_Expr = bind_discard_L (parse_keyword "(")
+                        (bind (parse_Expr n') (\x ->
+                          bind_discard_L (parse_keyword ")") (pure x)))}
+    in
+    let {
+     parse_Simple = alternative
+                      (alternative
+                        (alternative
+                          (alternative
+                            (alternative
+                              (alternative
+                                (alternative parse_Sub_Expr parse_Var)
+                                (parse_Lambda (parse_Expr n'))) parse_Bool)
+                            parse_Nat) (parse_Cond (parse_Expr n')))
+                        (parse_Let (parse_Expr n')))
+                      (parse_Eq (parse_Expr n'))}
+    in
+    let {
+     parse_Complex = alternative
+                       (alternative
+                         (alternative (alternative parse_Add parse_Sub)
+                           parse_Mul) parse_And) parse_Apply}
+    in
+    alternative
+      (bind parse_Simple (\x ->
+        bind parse_Complex (\op -> bind parse_Simple (\y -> pure (op x y)))))
+      parse_Simple)
+    n
+
+execute :: Prelude.String -> Env -> Prelude.Integer -> Prelude.Either
+           (([]) Prelude.String) Value
+execute s e max =
+  case parse
+         (parse_Expr (Prelude.succ (Prelude.succ (Prelude.succ (Prelude.succ
+           (Prelude.succ (Prelude.succ (Prelude.succ (Prelude.succ
+           (Prelude.succ (Prelude.succ 0))))))))))) s of {
+   Prelude.Left err -> Prelude.Left err;
+   Prelude.Right p ->
+    case p of {
+     (,) f _ ->
+      case eval f e max of {
+       Prelude.Left err -> Prelude.Left (snd err);
+       Prelude.Right v -> Prelude.Right v}}}
+
+input_vars :: (([]) ((,) Prelude.String Prelude.Integer)) -> Env
+input_vars assignments =
+  fold_right (\assignment env ->
+    case assignment of {
+     (,) x n -> ExtendEnv x (V_Nat n) env}) EmptyEnv assignments
+
+mult_str :: Prelude.String
+mult_str =
+  "Let mult := \\n -> \\m -> n * m In (mult . ione) . itwo"
+
+parse_mult :: Prelude.Either (([]) Prelude.String)
+              ((,) Expr (([]) Prelude.String))
+parse_mult =
+  parse
+    (parse_Expr (Prelude.succ (Prelude.succ (Prelude.succ (Prelude.succ
+      (Prelude.succ (Prelude.succ (Prelude.succ (Prelude.succ (Prelude.succ
+      (Prelude.succ 0))))))))))) mult_str
+
+double_str :: Prelude.String
+double_str =
+  "Let double := \\n -> n * 2 In double . input"
+
+parse_double :: Prelude.Either (([]) Prelude.String)
+                ((,) Expr (([]) Prelude.String))
+parse_double =
+  parse
+    (parse_Expr (Prelude.succ (Prelude.succ (Prelude.succ (Prelude.succ
+      (Prelude.succ (Prelude.succ (Prelude.succ (Prelude.succ (Prelude.succ
+      (Prelude.succ 0))))))))))) double_str
+
+parse_double_exec :: Prelude.Either (([]) Prelude.String) Value
+parse_double_exec =
+  execute double_str
+    (input_vars ((:) ((,) "input" (Prelude.succ (Prelude.succ (Prelude.succ
+      (Prelude.succ (Prelude.succ (Prelude.succ (Prelude.succ (Prelude.succ
+      (Prelude.succ (Prelude.succ 0))))))))))) ([]))) (Prelude.succ
+    (Prelude.succ (Prelude.succ (Prelude.succ (Prelude.succ (Prelude.succ
+    (Prelude.succ (Prelude.succ (Prelude.succ (Prelude.succ (Prelude.succ
+    (Prelude.succ (Prelude.succ (Prelude.succ (Prelude.succ (Prelude.succ
+    (Prelude.succ (Prelude.succ (Prelude.succ (Prelude.succ (Prelude.succ
+    (Prelude.succ (Prelude.succ (Prelude.succ (Prelude.succ (Prelude.succ
+    (Prelude.succ (Prelude.succ (Prelude.succ (Prelude.succ (Prelude.succ
+    (Prelude.succ (Prelude.succ (Prelude.succ (Prelude.succ (Prelude.succ
+    (Prelude.succ (Prelude.succ (Prelude.succ (Prelude.succ (Prelude.succ
+    (Prelude.succ (Prelude.succ (Prelude.succ (Prelude.succ (Prelude.succ
+    (Prelude.succ (Prelude.succ (Prelude.succ (Prelude.succ
+    0))))))))))))))))))))))))))))))))))))))))))))))))))
+
+factorial_str :: Prelude.String
+factorial_str =
+  "Let factorial :=\n      \\n ->\n        If {n == 1}\n        Then 1\n        Else n * (factorial . (n - 1))\n     In\n     factorial . input"
+
+parse_factorial :: Prelude.Either (([]) Prelude.String)
+                   ((,) Expr (([]) Prelude.String))
+parse_factorial =
+  parse
+    (parse_Expr (Prelude.succ (Prelude.succ (Prelude.succ (Prelude.succ
+      (Prelude.succ (Prelude.succ (Prelude.succ (Prelude.succ (Prelude.succ
+      (Prelude.succ 0))))))))))) factorial_str
+
+parse_factorial_exec :: Prelude.Either (([]) Prelude.String) Value
+parse_factorial_exec =
+  execute factorial_str
+    (input_vars ((:) ((,) "input" (Prelude.succ (Prelude.succ (Prelude.succ
+      (Prelude.succ (Prelude.succ 0)))))) ([]))) (Prelude.succ (Prelude.succ
+    (Prelude.succ (Prelude.succ (Prelude.succ (Prelude.succ (Prelude.succ
+    (Prelude.succ (Prelude.succ (Prelude.succ (Prelude.succ (Prelude.succ
+    (Prelude.succ (Prelude.succ (Prelude.succ (Prelude.succ (Prelude.succ
+    (Prelude.succ (Prelude.succ (Prelude.succ (Prelude.succ (Prelude.succ
+    (Prelude.succ (Prelude.succ (Prelude.succ (Prelude.succ (Prelude.succ
+    (Prelude.succ (Prelude.succ (Prelude.succ (Prelude.succ (Prelude.succ
+    (Prelude.succ (Prelude.succ (Prelude.succ (Prelude.succ (Prelude.succ
+    (Prelude.succ (Prelude.succ (Prelude.succ (Prelude.succ (Prelude.succ
+    (Prelude.succ (Prelude.succ (Prelude.succ (Prelude.succ (Prelude.succ
+    (Prelude.succ (Prelude.succ (Prelude.succ
+    0))))))))))))))))))))))))))))))))))))))))))))))))))
+
