theories/Examples.v
@@ -1,4 +1,9 @@
 From Coq Require Import Strings.String.
+From Coq Require Import Lists.List. Import ListNotations.
+From Coq Require Import Extraction.
+From Coq Require Import ExtrHaskellBasic.
+From Coq Require Import ExtrHaskellString.
+From Coq Require Import ExtrHaskellNatNum.
 Require Import Syntax.
 Require Import Semantics.
 Require Import Parser.
@@ -7,24 +12,33 @@ Module Examples.
 
   Import Syntax.
   Import Semantics.
+  Import Parser.
 
   Open Scope string_scope.
 
-  Example factorial :=
-    F_Let "factorial"
-      (F_Lambda "n"
-        (F_Cond
-          (B_Eq (E_Arith (A_Var "n")) (E_Arith (A_Const 1)))
-          (F_Return (E_Arith (A_Const 1)))
-          (F_Return (E_Arith (A_Mul
-                      (A_Func (F_Var "n"))
-                      (A_Func (F_Apply (F_Var "factorial") (F_Return (E_Arith (A_Sub (A_Func (F_Var "n")) (A_Const 1)))))))))))
-      (F_Apply (F_Var "factorial") (F_Return (E_Arith (A_Func (F_Var "input"))))).
+  Example mult_str :=
+    "Let mult := \n -> \m -> n * m In (mult . ione) . itwo".
+  Example parse_mult := parse (parse_Expr 10) mult_str.
+  Compute parse (parse_Expr 10) mult_str.
 
-  Example factorial_eval (n : nat) :=
-    Feval factorial (ExtendEnv "input" (V_Nat n) EmptyEnv) 1000.
+  Example double_str :=
+    "Let double := \n -> n * 2 In double . input".
+  Example parse_double := parse (parse_Expr 10) double_str.
+  Compute parse_double.
+  Example parse_double_exec := execute double_str (input_vars [("input", 10)]) 50.
 
-  Compute factorial_eval.
+  Example factorial_str :=
+    "Let factorial :=
+      \n ->
+        If {n == 1}
+        Then 1
+        Else n * (factorial . (n - 1))
+     In
+     factorial . input".
+  Example parse_factorial := parse (parse_Expr 10) factorial_str.
+  Compute parse_factorial.
+  Example parse_factorial_exec := execute factorial_str (input_vars [("input", 5)]) 50.
+  Compute parse_factorial_exec.
 
 End Examples.
 
@@ -42,6 +56,10 @@ Extract Inductive nat => "Prelude.Integer" ["0" "Prelude.succ"]
   "(\fO fS n -> if n Prelude.== 0 then fO () else fS (n Prelude.- 1))".
 
 Extraction
-  "Examples.hs"
-  factorial_eval
-  test_ex_hask_parse.
+  "extr/Examples.hs"
+  parse_mult
+  parse_double
+  parse_double_exec
+  parse_factorial
+  parse_factorial_exec
+  execute.
